src/MemoryPerms.v
@@ -18,19 +18,13 @@ From Heapster Require Import
      Permissions
      Memory
      SepStep
-     Typing.
+     Typing
+     PermType
+     PermTypeProofs.
 
 From ITree Require Import
      ITree
-     ITreeFacts
-     Basics.MonadState
-     Basics.MonadProp
-     Events.State
-     Events.Exception
-     Events.Nondeterminism
-     Eq.Eqit
-     Eq.UpToTaus
-     Eq.EqAxiom.
+     Eq.Eqit.
 
 From Paco Require Import
      paco.
@@ -38,6 +32,7 @@ From Paco Require Import
 Import MonadNotation.
 Import ListNotations.
 Import ITreeNotations.
+
 Local Open Scope itree_scope.
 (* end hide *)
 
@@ -154,18 +149,19 @@ Section MemoryPerms.
   (** Gives permission to allocate memory, assuming the last allocated block was [n-1] *)
   Program Definition malloc_perm (n : nat) : (@perm (Si * Ss)) :=
     {|
-    (** always valid *)
-    pre '(x, _) := length (lget x) = n;
-    (** No new blocks are allocated *)
-    rely '(x, _) '(y, _) := length (lget x) = length (lget y) /\
-                            (forall ptr, fst ptr >= n ->
-                                    sizeof (lget x) ptr = sizeof (lget y) ptr /\
-                                    read (lget x) ptr = read (lget y) ptr);
-    (** Existing blocks do not change *)
-    guar '(x, _) '(y, _) :=
+      (** always valid *)
+      pre '(x, _) := length (lget x) = n;
+      (** No new blocks are allocated *)
+      rely '(x, _) '(y, _) := length (lget x) = length (lget y) /\
+                                (forall ptr, fst ptr >= n ->
+                                        sizeof (lget x) ptr = sizeof (lget y) ptr /\
+                                          read (lget x) ptr = read (lget y) ptr);
+      (** Existing blocks do not change *)
+      guar '(x, _) '(y, _) :=
+      (exists z, y = lput x z) /\
       (forall ptr, fst ptr < n ->
               read (lget x) ptr = read (lget y) ptr /\
-              sizeof (lget x) ptr = sizeof (lget y) ptr);
+                sizeof (lget x) ptr = sizeof (lget y) ptr);
     |}.
   Next Obligation.
     constructor; [intros [] | intros [] [] []]; auto. intros [] [].
@@ -173,8 +169,11 @@ Section MemoryPerms.
       (etransitivity; [apply H0 | apply H2]; eauto).
   Qed.
   Next Obligation.
-    constructor; [intros [] | intros [] [] [] ? ?]; auto.
-    split; (etransitivity; [apply H; auto |]); apply H0; auto.
+    constructor; [intros [] | intros [] [] [] [] []]; auto.
+    - split; auto. eexists. symmetry. apply lPutGet.
+    - split.
+      + destruct H, H1. subst. eexists. rewrite lPutPut. reflexivity.
+      + intros. split; (etransitivity; [apply H0 | apply H2]; auto).
   Qed.
 
   Program Definition block_perm (size : nat) (ptr : addr) : (@perm (Si * Ss)) :=
@@ -203,7 +202,7 @@ Section MemoryPerms.
     malloc_perm n ⊥ block_perm size ptr.
   Proof.
     intros Hsize Hn.
-    constructor; intros [] [] ?; simpl in *; subst; auto.
+    constructor; intros [] [] ?; cbn in *; subst; auto.
     intros. apply H; auto.
   Qed.
 
@@ -230,31 +229,41 @@ Section MemoryPerms.
     (* only checks if the memory [ptr] points to in the 2 configs are equal *)
     rely '(x, _) '(y, _) := read (lget x) ptr = read (lget y) ptr;
     (* only the pointer we have write permission to may change *)
-    guar '(x, _) '(y, _) := (forall ptr', ptr <> ptr' -> read (lget x) ptr' = read (lget y) ptr') /\
-                            (forall ptr', sizeof (lget x) ptr' = sizeof (lget y) ptr') /\
-                            length (lget x) = length (lget y);
+      guar '(x, _) '(y, _) :=
+      (exists z, y = lput x z) /\
+        (forall ptr', ptr <> ptr' -> read (lget x) ptr' = read (lget y) ptr') /\
+        (forall ptr', sizeof (lget x) ptr' = sizeof (lget y) ptr') /\
+        length (lget x) = length (lget y);
     |}.
   Next Obligation.
     constructor; [intros [] | intros [] [] []]; auto; etransitivity; eauto.
   Qed.
   Next Obligation.
     constructor; [intros [] |]; auto.
-    intros [] [] [] ? ?.
-    split; [| split]; (etransitivity; [apply H; auto |]); apply H0; auto.
+    - split; auto. eexists. symmetry. apply lPutGet.
+    - intros [] [] [] [] []. split.
+      + destruct H, H1. subst. eexists. rewrite lPutPut. reflexivity.
+      + split; [| split]; (etransitivity; [apply H0; auto |]); apply H2; auto.
   Qed.
 
+  Lemma read_separate ptr ptr' v v' :
+    read_perm ptr v ⊥ read_perm ptr' v'.
+  Proof.
+    split; intros; auto; destruct x, y; cbn in *; subst; reflexivity.
+  Qed.
 
   Lemma read_lte_write : forall ptr v, read_perm ptr v <= write_perm ptr v.
   Proof.
-    constructor; simpl; intros [] []; subst; auto. intros; subst.
-    split; [| split]; reflexivity.
+    constructor; cbn; intros [] []; subst; auto. intros; subst.
+    split; [| split; [| split]]; try reflexivity.
+    eexists. symmetry. apply lPutGet.
   Qed.
 
   Lemma malloc_write : forall n ptr v,
       fst ptr < n ->
       malloc_perm n ⊥ write_perm ptr v.
   Proof.
-    intros n ptr v. constructor; intros [] []; simpl in *; intros.
+    intros n ptr v. constructor; intros [] []; cbn in *; intros.
     - destruct ptr. split; [| intros [] ?; split]; auto; apply H0;
                       intro Heq; inversion Heq; subst; lia.
     - apply H0; auto.
@@ -263,7 +272,7 @@ Section MemoryPerms.
   Lemma write_block : forall b o o' size v,
       block_perm size (b, o) ⊥ write_perm (b, o') v.
   Proof.
-    constructor; intros [] [] ?; simpl in *; subst; auto.
+    constructor; intros [] [] ?; cbn in *; subst; auto.
     apply H.
   Qed.
 
@@ -271,10 +280,10 @@ Section MemoryPerms.
       ptr <> ptr' ->
       write_perm ptr v ⊥ write_perm ptr' v'.
   Proof.
-    intros Hdiff. constructor; intros; destruct x, y; simpl; apply H; auto.
+    intros Hdiff. constructor; intros; destruct x, y; cbn; apply H; auto.
   Qed.
 
-  Program Definition post_malloc_perm n size : @perm (Si * Ss) :=
+  Program Definition post_malloc_perm' n size : @perm (Si * Ss) :=
     {|
     pre '(x, _) :=
       length (lget x) = n + 1 /\
@@ -288,20 +297,22 @@ Section MemoryPerms.
     guar_PO := guar_PO (malloc_perm (n + 1) ** block_perm size (n, 0) ** write_perm (n, 0) (VNum 0));
     |}.
 
-  Lemma sep_step_malloc n size : sep_step (malloc_perm n)
-                                          (post_malloc_perm n size).
+  Lemma sep_step_malloc' n size : sep_step (malloc_perm n)
+                                          (post_malloc_perm' n size).
   Proof.
     apply sep_step_rg.
     - intros [si ss] [si' ss'] ?. induction H; try solve [etransitivity; eauto].
       destruct H.
-      2: { destruct x, y. destruct H as (? & ? & ?). split; auto.
-           apply H; intro Heq; inversion Heq; subst; simpl in *; lia.
+      2: { destruct x, y. destruct H as (? & ? & ? & ?). split. apply H.
+           split; auto.
+           apply H0; intro Heq; inversion Heq; subst; cbn in *; lia.
       }
       induction H; try solve [etransitivity; eauto]. destruct H.
-      + destruct x, y. split; apply H; lia.
-      + destruct x, y. simpl in *. subst; auto.
+      + destruct x, y. split. apply H. split; apply H; lia.
+      + destruct x, y. cbn in *. subst; split; auto.
+        eexists. symmetry. apply lPutGet.
     - intros [si ss] [si' ss'] [Hlen Hptr]. simpl in *.
-      split; [split; [split |] |]; auto; intros; apply Hptr; simpl; lia.
+      split; [split; [split |] |]; auto; intros; apply Hptr; cbn; lia.
   Qed.
 
   (* Lemma read_write_separate_neq_ptr : forall ptr ptr' v v', *)
@@ -352,60 +363,6 @@ Section MemoryPerms.
   Definition write_Perms (ptr : addr) (P : Value -> Perms) : Perms :=
     meet_Perms (fun Q => exists y : Value, Q = singleton_Perms (write_perm ptr y) * P y).
 
-  (** * Memory operations *)
-  Definition load (v : Value) : itree (sceE Si) Value :=
-    s <- trigger (Modify id);;
-    match v with
-    | VNum _ => throw tt
-    | VPtr p => match read (lget s) p with
-               | None => throw tt
-               | Some b => Ret b
-               end
-    end.
-
-  Definition store (ptr : Value) (v : Value) : itree (sceE Si) Si :=
-    match ptr with
-    | VNum _ => throw tt
-    | VPtr ptr => s <- trigger (Modify (fun s => match write (lget s) ptr v with
-                                            | None => s
-                                            | Some c => (lput s c)
-                                            end)) ;;
-                 match write (lget s) ptr v with
-                 | None => throw tt
-                 | Some c => Ret (lput s c)
-               end
-    end.
-
-  Definition malloc (size : nat) : itree (sceE Si) Value :=
-    s <- trigger (Modify id);; (* do a read first to use length without subtraction *)
-    trigger (Modify (fun s =>
-                       (lput s ((lget s) ++
-                                         [Some (LBlock size
-                                                       (fun o => if o <? size
-                                                              then Some (VNum 0)
-                                                              else None))]))));;
-    Ret (VPtr (length (lget s), 0)).
-
-  Definition free (ptr : Value) : itree (sceE Si) unit :=
-    match ptr with
-    | VNum _ => throw tt
-    | VPtr ptr =>
-      if snd ptr =? 0
-      then
-        s <- trigger (Modify id);;
-        match nth_error (lget s) (fst ptr) with
-        | Some (Some (LBlock size bytes)) =>
-          trigger (Modify (fun s =>
-                             (lput s (replace_list_index
-                                        (lget s)
-                                        (fst ptr)
-                                        (Some (LBlock size (fun o => if o <? size then None else bytes o)))))));;
-          Ret tt
-        | _ => throw tt
-        end
-      else throw tt
-    end.
-
   Example no_error_load s : no_errors (lput s (mem_at (0, 0) (VNum 1)))
                                       (load (VPtr (0, 0))).
   Proof.
@@ -437,27 +394,28 @@ Section MemoryPerms.
     rewritebisim @bind_trigger. econstructor; eauto; try reflexivity.
     (* write step *)
     rewritebisim @bind_trigger. unfold id. econstructor; eauto.
-    { apply Hp in Hpre. apply Hp. simpl in *. rewrite lGetPut.
-      intros ptr Hn. split.
-      - unfold read, allocated. simpl. subst. rewrite nth_error_app_early; auto.
-      - unfold sizeof. simpl. subst. rewrite nth_error_app_early; auto.
+    { apply Hp in Hpre. apply Hp. cbn in *. rewrite lGetPut. split.
+      - eexists. reflexivity.
+      - intros ptr Hn. split.
+        + unfold read, allocated. cbn. subst. rewrite nth_error_app_early; auto.
+        + unfold sizeof. cbn. subst. rewrite nth_error_app_early; auto.
     }
     (* return *)
-    { eapply sep_step_lte. apply Hp. apply sep_step_malloc. }
+    { eapply sep_step_lte. apply Hp. apply sep_step_malloc'. }
     { econstructor; eauto.
-      - simpl. repeat rewrite lGetPut. apply Hp in Hpre. simpl in Hpre.
+      - cbn. repeat rewrite lGetPut. apply Hp in Hpre. cbn in Hpre.
         split; [| split].
         + rewrite last_length. lia.
-        + unfold sizeof. simpl.
+        + unfold sizeof. cbn.
           rewrite nth_error_app_last; auto.
-        + unfold read, allocated. simpl. rewrite nth_error_app_last; auto.
-      - simpl. apply Hp in Hpre. simpl in Hpre. rewrite Hpre.
+        + unfold read, allocated. cbn. rewrite nth_error_app_last; auto.
+      - cbn. apply Hp in Hpre. rewrite Hpre.
         eexists. exists (write_perm (n, 0) (VNum 0)).
         split; [| split; [| split]].
         + do 2 eexists. split; [| split; [| split]]; try reflexivity.
           1: eexists; split.
           * exists (n + 1). reflexivity.
-          * simpl. reflexivity.
+          * cbn. reflexivity.
           * apply malloc_block; cbn; lia.
         + eexists. split; [exists (VNum 0); reflexivity |].
           do 2 eexists. split; [cbn; reflexivity | split; [| split]]; cbn; auto.
@@ -468,17 +426,18 @@ Section MemoryPerms.
           * symmetry. apply write_block.
           * symmetry. apply malloc_block; cbn; lia.
         + constructor; auto.
-          { intros [] (? & ? & ?). simpl in *. split; split; auto.
-            - split; [| apply malloc_block; simpl; lia].
+          { intros [] (? & ? & ?). cbn in *. split; split; auto.
+            - split; [| apply malloc_block; cbn; lia].
               apply H0.
             - symmetry. apply separate_sep_conj_perm; symmetry.
-              + apply malloc_write. simpl. lia.
+              + apply malloc_write. cbn. lia.
               + apply write_block.
-              + apply malloc_block; simpl; lia.
+              + apply malloc_block; cbn; lia.
           }
     }
   Qed.
 
+  (*
   Lemma typing_free ptr (Q : Value -> Perms) :
     typing
       (write_Perms ptr Q * singleton_Perms (block_perm 1 ptr))
@@ -509,7 +468,7 @@ Section MemoryPerms.
     rewritebisim @bind_trigger. unfold id. econstructor; auto.
     - apply Hlte. constructor 1. left.
       apply Hlte'. constructor 1. left.
-      apply Hpwrite. simpl.
+      apply Hpwrite. cbn.
       split; [| split]; rewrite lGetPut; simpl; auto.
       + intros. unfold read. unfold allocated. simpl.
         destruct ptr as [b o]; destruct ptr' as [b' o'].
@@ -522,6 +481,7 @@ Section MemoryPerms.
     - apply sep_step_lte'. apply bottom_perm_is_bottom.
     - constructor; simpl; auto.
   Admitted.
+   *)
 
   (* Lemma typing_load {R} ptr (Q : Value -> Perms) (r : R) : *)
   (*   typing *)
@@ -552,7 +512,7 @@ Section MemoryPerms.
     intros p'' c1 c2 H Hpre. pstep. unfold store. rewritebisim @bind_trigger.
     destruct H as (p' & q & Hwrite & Hq & Hsep & Hlte).
     destruct Hwrite as (? & (v & ?) & Hwrite); subst.
-    destruct Hwrite as (pw & p & Hwritelte & Hp & Hsep' & Hlte'). simpl in *.
+    destruct Hwrite as (pw & p & Hwritelte & Hp & Hsep' & Hlte'). cbn in *.
     assert (exists val, read (lget c1) ptr = Some val).
     {
       apply Hlte in Hpre. destruct Hpre as (Hpre & _).
@@ -563,9 +523,10 @@ Section MemoryPerms.
     destruct Hread as (c' & Hwrite).
     assert (Hguar : guar p' (c1, c2) ((lput c1 c'), c2)).
     {
-      apply Hlte'. constructor 1. left. apply Hwritelte. simpl.
+      apply Hlte'. constructor 1. left. apply Hwritelte. cbn.
       rewrite lGetPut.
-      split; [| split].
+      split; [| split; [| split]].
+      + eexists. reflexivity.
       + eapply write_success_read_neq; eauto.
       + eapply write_success_sizeof; eauto.
       + rewrite lGetPut. eapply write_success_length; eauto.
@@ -609,4 +570,981 @@ Section MemoryPerms.
   (*   rewrite H. apply typing_store. *)
   (* Qed. *)
 
+  Definition offset (v : Value) (o : nat) : Value :=
+    match v with
+    | VNum n => VNum (n + o)
+    | VPtr (blk, n) => VPtr (blk, n + o)
+    end.
+
+  Definition ptr_Perms {A} (rw : RW) (p : Value) (a : A) (T : VPermType A) : @Perms (Si * Ss) :=
+    match p with
+    | VNum _ => top_Perms
+    | VPtr p =>
+        meet_Perms (fun P => exists (v : Value), P = singleton_Perms (match rw with
+                                                    | R => read_perm p v
+                                                    | W => write_perm p v
+                                                    end) *
+                                     (v :: T ▷ a))
+    end.
+
+  Definition ptr {A} '(rw, o, T) : VPermType A :=
+    {|
+      ptApp := fun x a => ptr_Perms rw (offset x o) a T;
+    |}.
+
+  Fixpoint arr_perm {A} rw o l T : VPermType (Vector.t A l) :=
+    match l with
+    | 0 => trueP
+    | S l' =>
+        {| ptApp := fun xi xss =>
+                      xi :: ptr (rw, o, T) ▷ Vector.hd xss *
+                        xi :: arr_perm rw (S o) l' T ▷ Vector.tl xss
+        |}
+    end.
+  Notation "'arr' ( rw , o , l , T )" := (arr_perm rw o l T).
+
+  Definition blockPT l : VPermType unit :=
+    {| ptApp := fun a _ => match a with
+                        | VPtr ptr => singleton_Perms (block_perm l ptr)
+                        | _ => top_Perms
+                        end |}.
+
+  Lemma reach_perm_proper {A} r (T : VPermType A) rw o :
+    Proper (lte_PermType ==> lte_PermType)
+           (fun U : VPermType (list A) => or (eqp r) (T ⋆ (ptr (rw, o, U)))).
+  Proof.
+    intros T1 T2 Hlte v l p Hp. cbn.
+    destruct l as [| ?]; cbn in *; auto.
+    destruct Hp as (pt & pptr & Hpt & Hpptr & Hlte').
+    exists pt, pptr. split; [| split]; auto.
+    clear Hpt. unfold ptr_Perms in *.
+    destruct (offset v o) as [? | l]; auto.
+    destruct Hpptr as (? & (v' & ?) & Hpptr); subst.
+    destruct Hpptr as (? & ? & ? & ? & ?).
+    eexists. split; eauto. do 2 eexists. split; [| split]; eauto. apply Hlte. auto.
+  Qed.
+
+  Program Definition reach_perm {A}
+          (r : Value) (rw : RW) (o : nat)
+          (T : VPermType A)
+    : VPermType (list A) :=
+    @mu _ _ _ (mu_list A) _ (fixed_point_list _)
+        (fun U => or (eqp r) (T ⋆ (ptr (rw, o, U))))
+        (reach_perm_proper _ _ _ _).
+
+  Program Definition list_perm rw A (T : VPermType A) : VPermType (list A) :=
+    @mu _ _ _ (mu_list A) _ (fixed_point_list _) (fun U => or (eqp (VNum 0)) (ptr (rw, 0, T) ⋆ ptr (rw, 1, U))) _.
+  Next Obligation.
+    repeat intro. cbn. induction b; cbn in *; auto.
+    destruct H0 as (? & ? & ? & ? & ? & ?). exists x0, x1. split; [| split]; auto.
+    clear H0. unfold ptr_Perms in *. destruct (offset a 1); auto.
+    destruct H1. destruct H0 as ((? & ?) & ?). subst. destruct H1 as (? & ? & ? & ? & ?).
+    eexists. split; eauto. do 2 eexists. split; eauto. split; eauto. apply H. auto.
+  Qed.
+
+  Definition list_reach_perm {A} r rw (T : VPermType A) : VPermType (list A) :=
+    reach_perm r rw 1 (ptr (rw, 0, T)).
+
+  Lemma reach_refl {A} x rw o (T : VPermType A) :
+    x :: trueP ▷ tt ⊨ x :: reach_perm x rw o T ▷ nil.
+  Proof.
+    repeat intro. apply mu_fixed_point. reflexivity.
+  Qed.
+
+  Lemma reach_trans {A} x y z rw o (T : VPermType A) xs ys :
+    x :: reach_perm y rw o T ▷ xs * y :: reach_perm z rw o T ▷ ys ⊨
+                                     x :: reach_perm z rw o T ▷ (xs ++ ys).
+  Proof.
+    revert x.
+    induction xs.
+    - intros x p (p1 & p2 & Hp1 & Hp2 & Hsep & Hlte).
+      destruct Hp1 as (? & (U & HU & ?) & Hp1); subst.
+      apply HU in Hp1. cbn in Hp1. subst. eapply Perms_upwards_closed; eauto.
+      etransitivity; eauto. apply lte_r_sep_conj_perm.
+    - intros x p (px' & py & Hpx' & Hpy & Hsep & Hlte).
+      eapply mu_fixed_point in Hpx'.
+      destruct Hpx' as (pa & px & Hpa & Hpx & Hsep' & Hlte').
+      (* x must be a pointer *)
+      destruct x; try contradiction. destruct a0 as [b o'].
+      destruct Hpx as (? & (v & ?) & Hpx); subst.
+      destruct Hpx as (px'' & pv & Hpx'' & Hpv & Hsep'' & Hlte'').
+
+      apply mu_fixed_point. cbn.
+      exists pa, (px'' ** (pv ** py)). split; [apply Hpa | split; [| split]].
+      3: { repeat rewrite <- sep_conj_perm_assoc.
+           etransitivity; eauto.
+           eapply sep_conj_perm_monotone; intuition.
+           repeat rewrite sep_conj_perm_assoc.
+           etransitivity; eauto.
+           eapply sep_conj_perm_monotone; intuition.
+      }
+      2: {
+        apply separate_sep_conj_perm.
+        - eapply separate_antimonotone; eauto.
+          etransitivity; eauto. apply lte_l_sep_conj_perm.
+        - apply separate_sep_conj_perm.
+          + eapply separate_antimonotone; eauto.
+            etransitivity; eauto. apply lte_r_sep_conj_perm.
+          + symmetry. symmetry in Hsep. eapply separate_antimonotone; eauto.
+            etransitivity; eauto. apply lte_l_sep_conj_perm.
+          + symmetry in Hsep. eapply separate_antimonotone; eauto.
+            etransitivity; eauto. etransitivity. apply lte_r_sep_conj_perm.
+            apply sep_conj_perm_monotone. reflexivity.
+            etransitivity; eauto. apply lte_r_sep_conj_perm.
+        - symmetry. apply separate_sep_conj_perm.
+          + eapply separate_antimonotone; eauto. reflexivity.
+          + symmetry. symmetry in Hsep. eapply separate_antimonotone; eauto.
+            etransitivity; eauto. etransitivity. apply lte_r_sep_conj_perm.
+            apply sep_conj_perm_monotone. reflexivity.
+            etransitivity; eauto. apply lte_l_sep_conj_perm.
+          + symmetry in Hsep. eapply separate_antimonotone; eauto.
+            etransitivity; eauto. etransitivity. apply lte_r_sep_conj_perm.
+            apply sep_conj_perm_monotone. reflexivity.
+            etransitivity; eauto. apply lte_r_sep_conj_perm.
+      }
+      eexists; split; [eexists; reflexivity |].
+      apply sep_conj_Perms_perm; [apply Hpx'' | |].
+      2: {
+        apply separate_sep_conj_perm; auto.
+        + symmetry. symmetry in Hsep. eapply separate_antimonotone; eauto.
+          etransitivity; eauto. etransitivity. apply lte_r_sep_conj_perm.
+          apply sep_conj_perm_monotone. reflexivity.
+          etransitivity; eauto. apply lte_l_sep_conj_perm.
+        + symmetry in Hsep. eapply separate_antimonotone; eauto.
+          etransitivity; eauto. etransitivity. apply lte_r_sep_conj_perm.
+          apply sep_conj_perm_monotone. reflexivity.
+          etransitivity; eauto. apply lte_r_sep_conj_perm.
+      }
+      cbn. exists (v :: reach_perm z rw o T ▷ (xs ++ ys)). split.
+      2: {
+        apply IHxs. apply sep_conj_Perms_perm; auto.
+        symmetry. symmetry in Hsep. eapply separate_antimonotone; eauto.
+        etransitivity; eauto. etransitivity. apply lte_r_sep_conj_perm.
+        apply sep_conj_perm_monotone. reflexivity.
+        etransitivity; eauto. apply lte_r_sep_conj_perm.
+      }
+      eexists; split; eauto.
+      repeat intro. eapply mu_fixed_point in H; auto.
+      Unshelve. all: apply reach_perm_proper.
+  Qed.
+
+  (** * Pointer rules *)
+
+  Lemma PtrI A xi yi xs ys rw o (T : @VPermType Si Ss A) :
+    xi :: ptr (rw, o, eqp yi) ▷ xs * yi :: T ▷ ys ⊨ xi :: ptr (rw, o, T) ▷ ys.
+  Proof.
+    destruct xi; cbn.
+    - rewrite sep_conj_Perms_top_absorb. reflexivity.
+    - repeat intro. destruct a. rename p into p'.
+      destruct H as (p & t & (P & (v & ?) & Hp) & Hp' & Hsep & Hlte). subst.
+      destruct Hp as (? & ? & ? & ? & Hsep' & Hlte'). cbn in *. subst.
+      eexists. split; [exists v; reflexivity |].
+      eapply Perms_upwards_closed; eauto.
+      do 2 eexists. split; [| split; [| split]]; eauto.
+      + symmetry. symmetry in Hsep. eapply separate_antimonotone; eauto.
+        etransitivity; eauto. apply lte_l_sep_conj_perm.
+      + apply sep_conj_perm_monotone; intuition.
+        etransitivity; eauto. apply lte_l_sep_conj_perm.
+  Qed.
+
+  Lemma PtrE A B C (P : Perms) rw o (T : @VPermType Si Ss A) (xi : Value) xs ti ts (U : @PermType Si Ss B C) :
+    (forall yi, P * xi :: ptr (rw, o, eqp yi) ▷ tt * yi :: T ▷ xs ⊢ ti ⤳ ts ::: U) ->
+    P * xi :: ptr (rw, o, T) ▷ xs ⊢ ti ⤳ ts ::: U.
+  Proof.
+    repeat intro. rename p into p''. destruct H0 as (p & p' & Hp & Hptr & Hsep & Hlte).
+    destruct xi; [contradiction | destruct a].
+    destruct Hptr as (? & (? & ?) & ?). subst.
+    destruct H2 as (pptr & pt & Hptr & Hpt & Hsep' & Hlte').
+    eapply H; eauto. exists (p ** pptr), pt.
+    split; [| split; [| split]]; eauto.
+    - do 2 eexists. split; [| split; [| split]]. eauto. 3: reflexivity.
+      + eexists. split; eauto. do 2 eexists.
+        split; [| split; [| split]]. eauto. reflexivity. 2: apply sep_conj_perm_bottom'.
+        apply separate_bottom.
+      + eapply separate_antimonotone; eauto. etransitivity; eauto. apply lte_l_sep_conj_perm.
+    - symmetry. symmetry in Hsep'. apply separate_sep_conj_perm; auto.
+      + symmetry. eapply separate_antimonotone; eauto. etransitivity; eauto.
+        apply lte_r_sep_conj_perm.
+      + symmetry. eapply separate_antimonotone; eauto. etransitivity; eauto.
+        apply lte_l_sep_conj_perm.
+    - etransitivity; eauto. rewrite sep_conj_perm_assoc.
+      apply sep_conj_perm_monotone; auto; reflexivity.
+  Qed.
+
+  Lemma ReadDup o xi yi :
+    xi :: ptr (R, o, eqp yi) ▷ tt ⊨
+       xi :: ptr (R, o, eqp yi) ▷ tt * xi :: ptr (R, o, eqp yi) ▷ tt.
+  Proof.
+    repeat intro. cbn in *. destruct xi; [contradiction |].
+    destruct a as [b o']. unfold offset in *.
+    destruct H as (? & (v & ?) & ?). subst.
+    exists (read_perm (b, o' + o) v), (read_perm (b, o' + o) v).
+    destruct H0 as (pread & peq & Hpread & Hpeq & Hsep & Hlte).
+    cbn in Hpread, Hpeq. subst.
+    assert (read_perm (b, o' + o) v ∈ ptr_Perms R (VPtr (b, o' + o)) tt (eqp v)).
+    {
+      eexists. split; eauto. cbn in *. exists (read_perm (b, o' + o) v), bottom_perm.
+      split; [| split; [| split]]. 2: reflexivity.
+      - split; intros; auto.
+      - apply separate_bottom.
+      - rewrite sep_conj_perm_bottom. reflexivity.
+    }
+    split; [| split; [| split]]; auto.
+    apply read_separate.
+    constructor; intros; eauto.
+    - split; [| split]; auto. 1, 2: apply Hpread; apply Hlte; auto.
+      apply read_separate.
+    - split; apply Hpread; apply Hlte; auto.
+    - apply Hlte. constructor. left. apply Hpread. induction H0; auto.
+      + destruct H0; auto.
+      + etransitivity; eauto.
+  Qed.
+
+  Lemma PtrOff A xi xs rw o1 o2 (T : @VPermType Si Ss A) :
+    o1 >= o2 ->
+    xi :: ptr (rw, o1, T) ▷ xs ⊨ offset xi o2 :: ptr (rw, o1 - o2, T) ▷ xs.
+  Proof.
+    destruct xi; [reflexivity | destruct a].
+    intros. cbn. rewrite <- Nat.add_assoc.
+    rewrite (Nat.add_comm o2 _). rewrite Nat.sub_add; auto.
+    reflexivity.
+  Qed.
+  Lemma PtrOff' A xi xs rw o1 o2 (T : @VPermType Si Ss A) :
+    o1 >= o2 ->
+    offset xi o2 :: ptr (rw, o1 - o2, T) ▷ xs ⊨ xi :: ptr (rw, o1, T) ▷ xs.
+  Proof.
+    destruct xi; [reflexivity | destruct a].
+    intros. cbn. rewrite <- Nat.add_assoc.
+    rewrite (Nat.add_comm o2 _). rewrite Nat.sub_add; auto.
+    reflexivity.
+  Qed.
+
+  Lemma Load xi yi xs rw :
+    xi :: ptr (rw, 0, eqp yi) ▷ xs ⊢
+       load xi ⤳
+       Ret tt :::
+       eqp yi ∅ xi :: ptr (rw, 0, eqp yi) ▷ xs.
+  Proof.
+    repeat intro. pstep. unfold load. rewritebisim @bind_trigger.
+    econstructor; eauto; try reflexivity.
+    destruct xi as [? | [b o]]; try contradiction.
+    cbn in H.
+    destruct H as (? & (v & ?) & ?); subst.
+    destruct H1 as (? & ? & ? & ? & Hsep & Hlte). cbn in H, H1. subst.
+    assert (read (lget c1) (b, o) = Some v).
+    {
+      apply Hlte in H0. destruct H0 as (? & _).
+      rewrite Nat.add_0_r in H. apply H in H0. destruct rw; auto.
+    }
+    rewrite H1. constructor; auto.
+    (* TODO: these exists are kind of weird *)
+    cbn. exists bottom_perm, x. split; [| split; [| split]]; auto.
+    - cbn. eexists. split; eauto.
+      cbn. exists x, bottom_perm. split; [| split; [| split]]; eauto.
+      apply separate_bottom.
+      rewrite sep_conj_perm_bottom. reflexivity.
+    - symmetry. apply separate_bottom.
+    - rewrite sep_conj_perm_commut. rewrite sep_conj_perm_bottom.
+      etransitivity; eauto. apply lte_l_sep_conj_perm.
+  Qed.
+
+  Lemma Store A xi yi xs (P : @VPermType Si Ss A) :
+    xi :: ptr (W, 0, P) ▷ xs ⊢
+       store xi yi ⤳
+       Ret tt :::
+       trueP ∅ xi :: ptr (W, 0, eqp yi) ▷ tt.
+  Proof.
+    repeat intro. pstep. unfold store. destruct xi as [| [b o]]; try contradiction.
+    rewritebisim @bind_trigger.
+    rename p into p'. rename H0 into Hpre.
+    destruct H as (? & (v & ?) & Hwrite); subst.
+    destruct Hwrite as (pw & p & Hwritelte & Hp & Hsep & Hlte).
+    rewrite Nat.add_0_r in Hwritelte.
+    assert (exists val, read (lget c1) (b, o) = Some val).
+    {
+      apply Hlte in Hpre. destruct Hpre as (Hpre & _).
+      apply Hwritelte in Hpre. eexists.
+      symmetry. apply Hpre.
+    }
+    destruct H as (val & Hread). eapply (read_success_write _ _ _ yi) in Hread.
+    destruct Hread as (c' & Hwrite).
+    assert (Hguar : guar p' (c1, c2) ((lput c1 c'), c2)).
+    {
+      apply Hlte. constructor 1. left. apply Hwritelte. cbn.
+      repeat rewrite lGetPut.
+      split; [| split; [| split]].
+      + eexists. reflexivity.
+      + eapply write_success_read_neq; eauto.
+      + eapply write_success_sizeof; eauto.
+      + eapply write_success_length; eauto.
+    }
+    econstructor; eauto.
+    3: {
+      rewrite Hwrite. constructor; eauto.
+      2: { cbn. exists bottom_perm. eexists. split; [| split; [| split]]; auto.
+           - eexists. split; eauto. cbn. eexists. exists bottom_perm.
+             split; [| split; [| split]]; eauto; try reflexivity.
+             apply separate_bottom.
+           - symmetry. apply separate_bottom.
+           - rewrite sep_conj_perm_bottom. rewrite sep_conj_perm_commut.
+             rewrite sep_conj_perm_bottom. reflexivity.
+      }
+      rewrite Nat.add_0_r. symmetry. eapply write_success_read_eq; rewrite lGetPut; eauto.
+    }
+    - rewrite Hwrite. auto.
+    - rewrite Nat.add_0_r. eapply sep_step_lte; eauto.
+      etransitivity.
+      + eapply sep_step_lte; [| reflexivity]. apply lte_l_sep_conj_perm.
+      + cbn in *. eapply sep_step_lte; eauto. intros ? []. constructor; auto.
+  Qed.
+
+  Lemma IsNull1 A xi xs rw o (P : @VPermType Si Ss A) :
+    xi :: ptr (rw, o, P) ▷ xs ⊢
+       isNull xi ⤳
+       Ret tt :::
+       eqp false ∅ xi :: ptr (rw, o, P) ▷ xs.
+  Proof.
+    repeat intro. pstep. unfold isNull. destruct xi; [contradiction |].
+    destruct a as [b o']. cbn. constructor; auto.
+    cbn. exists bottom_perm, p. split; [| split; [| split]]; eauto.
+    - symmetry. apply separate_bottom.
+    - rewrite sep_conj_perm_commut. rewrite sep_conj_perm_bottom. reflexivity.
+  Qed.
+
+  Lemma IsNull2 xi:
+    xi :: @eqp Si Ss _ (VNum 0) ▷ tt ⊢
+       isNull xi ⤳
+       Ret tt :::
+       eqp true.
+  Proof.
+    repeat intro. pstep. cbn in *. subst. constructor; cbn; auto.
+  Qed.
+
+  (*
+  (** * Example 2 *)
+  Definition ex2i xi yi : itree (sceE Si) Si :=
+    x <- load xi;;
+    store yi x.
+
+  Definition ex2s : itree (sceE Ss) unit :=
+    Ret tt ;;
+    Ret tt.
+
+  Lemma ex2_typing A (xi yi : Value) xs (T : @VPermType Si Ss A) :
+    xi :: ptr (R, 0, T) ▷ xs * yi :: ptr (W, 0, trueP) ▷ tt ⊢
+                                 ex2i xi yi ⤳
+                                 ex2s :::
+                                 trueP ∅ yi :: ptr (W, 0, T) ▷ xs ∅ xi :: ptr (R, 0, trueP) ▷ tt.
+  Proof.
+    (* PtrE *)
+    rewrite sep_conj_Perms_commut.
+    eapply PtrE; eauto; intros zi.
+    (* Bind *)
+    eapply Bind.
+    (* L: Frame and Load *)
+    apply Frame. rewrite sep_conj_Perms_commut. apply Frame. apply Load.
+    (* Weak *)
+    intros wi [].
+    eapply Weak with (P2 := yi :: ptr _ _ (W, 0, trueP _ _) ▷ tt *
+                              wi :: T ▷ xs *
+                              xi :: ptr _ _ (R, 0, trueP _ _) ▷ tt)
+                     (U2 := trueP _ _ ∅
+                                  yi :: ptr _ _ (W, 0, eqp _ _ wi) ▷ tt ∅
+                                  wi :: T ▷ xs ∅
+                                  xi :: ptr _ _ (R, 0, trueP _ _) ▷ tt).
+    (* Input type *)
+    - etransitivity.
+      (* PermsE *)
+      {
+        etransitivity; [apply PermsE |]. rewrite sep_conj_Perms_commut.
+        eapply sep_conj_Perms_monotone; [reflexivity |]. (* frame *)
+        etransitivity; [| apply PermsE]. rewrite sep_conj_Perms_commut.
+        eapply sep_conj_Perms_monotone; [reflexivity |]. (* frame *)
+        etransitivity; [| apply PermsE]. rewrite sep_conj_Perms_commut. reflexivity.
+      }
+      rewrite (sep_conj_Perms_commut (zi :: T ▷ xs) _).
+      repeat rewrite <- sep_conj_Perms_assoc.
+      apply sep_conj_Perms_monotone; [reflexivity |].
+      rewrite sep_conj_Perms_commut.
+      eapply sep_conj_Perms_monotone.
+      (* Weakening the content type *)
+      + etransitivity; [apply PtrI | apply TrueI].
+      (* Cast *)
+      + apply Cast.
+    (* Output type *)
+    - intros ? [].
+      etransitivity; [apply PermsE |].
+      etransitivity; [| apply PermsI].
+      eapply sep_conj_Perms_monotone; [| reflexivity]. (* frame *)
+      etransitivity; [| apply PermsE].
+      etransitivity; [apply PermsI |].
+      etransitivity.
+      2: {
+        eapply sep_conj_Perms_monotone; [| reflexivity]. (* frame *)
+        apply PermsE.
+      }
+      rewrite <- sep_conj_Perms_assoc.
+      eapply sep_conj_Perms_monotone; [reflexivity |]. (* frame *)
+      (* PtrI *)
+      apply PtrI.
+    (* Frame and Store *)
+    - apply Frame. apply Frame. apply Store.
+  Qed.
+
+   *)
+
+  (** * Array rules *)
+  Lemma ArrCombine_eq A xi rw o l1 l2 (l:le l2 l1) xs1 xs2 (P : @VPermType Si Ss A) :
+    eq_Perms (xi :: arr (rw, o, l1, P) ▷ append_leq l1 l2 l xs1 xs2)
+             (xi :: arr (rw, o, l2, P) ▷ xs1 * xi :: arr (rw, o + l2, l1 - l2, P) ▷ xs2).
+  Proof.
+    revert o l2 l xs1 xs2; induction l1; intros.
+    - inversion l. subst. cbn. rewrite sep_conj_Perms_bottom_identity. reflexivity.
+    - destruct l2.
+      + rewrite sep_conj_Perms_bottom_identity.
+        rewrite Nat.add_0_r. reflexivity.
+      + cbn. rewrite (IHl1 (S o) l2).
+        rewrite Nat.add_succ_r.
+        rewrite sep_conj_Perms_assoc.
+        reflexivity.
+  Qed.
+
+  Lemma ArrSplit A R1 R2 P l1 l2 xi xs rw o (T : @VPermType Si Ss A) U (ti : itree (sceE Si) R1) (fs : _ -> _ -> itree (sceE Ss) R2) :
+    (forall xs1 xs2, P *
+                  xi :: arr (rw, o, l2, T) ▷ xs1 *
+                  xi :: arr (rw, o + l2, l1 - l2, T) ▷ xs2 ⊢
+                     ti ⤳ fs xs1 xs2 ::: U) ->
+    P * xi :: arr (rw, o, l1, T) ▷ xs ⊢ ti ⤳ trySplit xs l2 fs ::: U.
+  Proof.
+    intros. unfold trySplit. destruct (Compare_dec.le_lt_dec l2 l1).
+    - rewrite <- (split_leq_append_leq _ l1 xs l2 l).
+      rewrite ArrCombine_eq. repeat rewrite split_leq_append_leq.
+      rewrite sep_conj_Perms_assoc.
+      apply H.
+    - apply Err.
+  Qed.
+
+  Lemma ArrCombine A xi rw o l1 l2 xs1 xs2 (P : @VPermType Si Ss A) :
+    xi :: arr (rw, o, l1, P) ▷ xs1 * xi :: arr (rw, o + l1, l2, P) ▷ xs2 ⊨
+    xi :: arr (rw, o, l1 + l2, P) ▷ Vector.append xs1 xs2 .
+  Proof.
+    repeat intro. destruct H as (p1 & p2 & Hp1 & Hp2 & Hsep & Hlte).
+    revert Hp1 Hp2. revert o xi l2 xs2. revert Hsep Hlte. revert p p1 p2. induction l1; intros.
+    - rewrite Nat.add_0_r in Hp2. cbn in *. revert xs1. apply Vector.case0. cbn.
+      eapply Perms_upwards_closed; eauto. etransitivity; [apply lte_r_sep_conj_perm |]; eauto.
+    - cbn. destruct Hp1 as (? & ? & ? & ? & Hsep' & Hlte').
+      do 2 eexists. split; [| split; [| split]].
+      + rewrite vector_hd_append. apply H.
+      + rewrite vector_tl_append. eapply IHl1. 2: reflexivity.
+        2: { eapply Perms_upwards_closed; eauto. reflexivity. }
+        2: { cbn. rewrite <- plus_n_Sm in Hp2. eauto. }
+        symmetry. symmetry in Hsep. eapply separate_antimonotone; eauto.
+        etransitivity; eauto. apply lte_r_sep_conj_perm.
+      + apply separate_sep_conj_perm; auto.
+        * symmetry. symmetry in Hsep. eapply separate_antimonotone; eauto.
+          etransitivity; eauto. apply lte_l_sep_conj_perm.
+        * symmetry in Hsep. eapply separate_antimonotone; eauto.
+          etransitivity; eauto. apply lte_r_sep_conj_perm.
+      + rewrite <- sep_conj_perm_assoc. etransitivity; eauto.
+        apply sep_conj_perm_monotone; eauto; reflexivity.
+  Qed.
+
+  Lemma ArrPtr A xi xs rw o (P : @VPermType Si Ss A) :
+    xi :: arr (rw, o, 1, P) ▷ xs ⊨ xi :: ptr (rw, o, P) ▷ Vector.hd xs.
+  Proof.
+    cbn. rewrite sep_conj_Perms_commut. rewrite sep_conj_Perms_bottom_identity. reflexivity.
+  Qed.
+
+  Lemma PtrArr A xi xs rw o (P : @VPermType Si Ss A) :
+    xi :: ptr (rw, o, P) ▷ xs ⊨ xi :: arr (rw, o, 1, P) ▷ vsingle xs.
+  Proof.
+    cbn. rewrite sep_conj_Perms_commut. rewrite sep_conj_Perms_bottom_identity. reflexivity.
+  Qed.
+
+  Lemma arr_offset {A} ptr rw o l (T : @VPermType Si Ss A) (v : Vector.t A l) :
+    VPtr ptr :: arr (rw, o, l, T) ▷ v ≡ offset (VPtr ptr) o :: arr (rw, 0, l, T) ▷ v.
+  Proof.
+    revert ptr o. induction l; intros ptr o; try reflexivity.
+    split.
+    - cbn. apply sep_conj_Perms_monotone.
+      + destruct ptr. cbn. rewrite Nat.add_0_r. reflexivity.
+      + destruct ptr. rewrite (IHl _ _ 1). cbn.
+        specialize (IHl (Vector.tl v) (n, n0) (o + 1)). cbn in IHl.
+        rewrite Nat.add_assoc in IHl. rewrite Nat.add_1_r in IHl. apply IHl.
+    - cbn. apply sep_conj_Perms_monotone.
+      + destruct ptr. cbn. rewrite Nat.add_0_r. reflexivity.
+      + destruct ptr. rewrite (IHl _ _ 1). cbn.
+        specialize (IHl (Vector.tl v) (n, n0) (o + 1)). cbn in IHl.
+        rewrite Nat.add_assoc in IHl. rewrite Nat.add_1_r in IHl. apply IHl.
+  Qed.
+
+  (** * Malloc *)
+  (** helper lemmas for Malloc *)
+  Fixpoint rely_post_malloc n b size x y : Prop :=
+    match n with
+    | 0 => rely (block_perm size (b, 0) ** malloc_perm (b + 1)) x y
+    | S n => rely (write_perm (b, size - S n) (VNum 0)) x y /\
+              rely_post_malloc n b size x y
+    end.
+  Lemma PO_rely_post_malloc n b size :
+    PreOrder (rely_post_malloc n b size).
+  Proof.
+    constructor.
+    - intros []; induction n; cbn; auto.
+    - intros [] [] [] ? ?. induction n.
+      + split; [| split]; try solve [etransitivity; [apply H | apply H0]].
+        intros; split; (etransitivity; [apply H | apply H0]); auto.
+      + split; try solve [etransitivity; [apply H | apply H0]].
+        apply IHn; [apply H | apply H0].
+  Qed.
+
+  Fixpoint guar_post_malloc n b size x y : Prop :=
+    match n with
+    | 0 => guar (block_perm size (b, 0) ** malloc_perm (b + 1)) x y
+    | S n => clos_trans _ (fun x y =>
+                            guar (write_perm (b, size - S n) (VNum 0)) x y \/
+                              guar_post_malloc n b size x y) x y
+    end.
+  #[local] Instance PO_guar_post_malloc n b size :
+    PreOrder (guar_post_malloc n b size).
+  Proof.
+    constructor.
+    - intros []. induction n; cbn; intuition.
+    - intros [] [] [] ? ?.
+      destruct n; econstructor 2; eauto.
+  Qed.
+
+  Definition pre_post_malloc n b size : Si * Ss -> Prop :=
+    fun '(x, _) =>
+      b + 1 = length (lget x) /\
+        Some size = sizeof (lget x) (b, 0) /\
+        forall o, o < size -> (size - n <= o)%nat -> Some (VNum 0) = read (lget x) (b, o).
+  Lemma pre_respects_post_malloc n b size :
+    forall x y, rely_post_malloc (S n) b size x y -> (* we need the fact that n > 0 here *)
+           pre_post_malloc (S n) b size x ->
+           pre_post_malloc (S n) b size y.
+  Proof.
+    intros [] [] Hrely (Hlen & Hsizeof & Hread).
+    cbn in *.
+    induction n; cbn in *.
+    - destruct Hrely as (Hread' & Hsizeof' & Hlen' & Hptr).
+      split; [rewrite <- Hlen' | split; [rewrite <- Hsizeof' |]]; auto.
+      intros. assert (o = size - 1) by lia. subst.
+      rewrite <- Hread'. auto.
+    - destruct Hrely as (Hread' & Head'' & Hrely). split; [| split].
+      + apply IHn; auto. intros. apply Hread; auto. lia.
+      + apply IHn; auto. intros. apply Hread; auto. lia.
+      + intros. assert (size - S (S n) = o \/ (size - S n <= o)%nat) by lia.
+        destruct H1.
+        * subst. rewrite <- Hread'. auto.
+        * apply IHn; auto. intros. apply Hread; auto. lia.
+  Qed.
+
+  (** The intermediate permission for Malloc. *)
+  (** [n] is the number of unfoldings to do for the rely/guar. [size] is the size of the block.
+    when we use this [n = size], but we need them separate to do induction on [n] *)
+  Program Definition post_malloc_perm n b size : @perm (Si * Ss) :=
+    {|
+      rely := rely_post_malloc (S n) b (S size);
+      rely_PO := PO_rely_post_malloc (S n) b (S size);
+      guar := guar_post_malloc (S n) b (S size);
+      guar_PO := PO_guar_post_malloc (S n) b (S size);
+      pre := pre_post_malloc (S n) b (S size);
+      pre_respects := pre_respects_post_malloc n b (S size); (* S is applied inside this defn *)
+    |}.
+
+  Lemma guar_malloc_post_malloc n b size x y :
+    guar_post_malloc n b (S size) x y -> guar (malloc_perm b) x y.
+  Proof.
+    revert x y. induction n; intros.
+    - induction H; try solve [etransitivity; eauto]. destruct H.
+      + destruct x, y. cbn in *. subst; split; auto.
+        eexists. symmetry. apply lPutGet.
+      + destruct x, y. split; [| split]; apply H; lia.
+    - induction H; auto.
+      + destruct H.
+        * destruct x, y. destruct H as (? & ? & ? & ?). split; [| split]; auto.
+          apply H0. destruct ptr0. intro. inversion H4. cbn in *. lia.
+        * apply IHn; auto.
+      + etransitivity; eauto.
+  Qed.
+
+  Lemma rely_malloc_post_malloc n b size x y :
+    rely (malloc_perm b) x y -> rely_post_malloc n b (S size) x y.
+  Proof.
+    destruct x, y. induction n; intros.
+    - destruct H as (Hlen & Hptr).
+      split; [| split]; simpl; auto.
+      + apply Hptr; auto.
+      + intros. apply Hptr; lia.
+    - split; auto. cbn in *. apply H. auto.
+  Qed.
+
+  Lemma sep_step_malloc n b size : sep_step (malloc_perm b)
+                                            (post_malloc_perm n b size).
+  Proof.
+    apply sep_step_rg.
+    - apply guar_malloc_post_malloc.
+    - apply rely_malloc_post_malloc.
+  Qed.
+
+  Lemma write_post_malloc_perm m n size b
+        (Hsize : (m <= size)%nat)
+        (Hm : m > n):
+    write_perm (b, size - m) (VNum 0) ⊥ post_malloc_perm n b size.
+  Proof.
+    constructor; auto; intros.
+    - revert H. revert x y. induction n; intros.
+      + induction H; try solve [etransitivity; eauto].
+        destruct H; [| induction H; try solve [etransitivity; eauto]; destruct H].
+        * eapply write_write_sep; eauto. intro. inversion H0. lia.
+        * eapply write_block; eauto.
+        * eapply malloc_write; eauto. rewrite Nat.add_1_r in H. auto.
+      + induction H; try solve [etransitivity; eauto].
+        destruct H. 2: apply IHn; auto; lia.
+        eapply write_write_sep; eauto. intro. inversion H0. lia.
+    - revert H. revert x y. induction n; intros.
+      + destruct x, y. split; [| split; [| split; [| split]]]; simpl in *; try apply H.
+        * intro. inversion H0. lia.
+        * destruct ptr0. intro. cbn in *. inversion H1. lia.
+      + destruct x, y. cbn in H. split; [| split]; cbn; try apply H.
+        * intro. inversion H0. lia.
+        * intro. inversion H0. lia.
+        * apply IHn. lia. auto.
+  Qed.
+
+  Lemma post_malloc_perm_extend b size n (Hn : (S n <= size)%nat) :
+    write_perm (b, size - S n) (VNum 0) ** post_malloc_perm n b size <=
+      post_malloc_perm (S n) b size.
+  Proof.
+    constructor; auto.
+    cbn in *; auto. intros [] H. destruct H as (Hlen & Hsizeof & Hread).
+    split; [| split; [split; [| split] |]]; auto; try solve [intros; apply Hread; lia].
+    apply write_post_malloc_perm; auto.
+  Qed.
+
+  Lemma post_malloc_perm_ok {A} n b size (xs : Vector.t A (S n))
+        (Hn : (n <= size)%nat) :
+    post_malloc_perm n b size (* the perm applies S to n and size inside *) ∈
+                     VPtr (b, size - n) :: arr_perm W 0 (S n) trueP ▷ xs *
+      singleton_Perms (block_perm (S size) (b, 0)) *
+      malloc_Perms.
+  Proof.
+    cbn. induction n.
+    - cbn. do 2 eexists. split; [| split; [| split]].
+      + do 2 eexists. split; [| split; [| split]]; try reflexivity.
+        * eexists. exists bottom_perm. split; [| split; [| split]]; auto. 3: reflexivity.
+          2: apply separate_bottom.
+          eexists. split; [exists (VNum 0); reflexivity |].
+          eexists. exists bottom_perm. split; [| split; [| split]]; cbn; try reflexivity.
+          apply separate_bottom.
+        * do 2 rewrite sep_conj_perm_bottom. symmetry. apply write_block.
+      + eexists. split; [exists (b + 1); reflexivity | cbn; reflexivity].
+      + do 2 rewrite sep_conj_perm_bottom. symmetry. apply separate_sep_conj_perm.
+        * apply malloc_write; cbn; lia.
+        * apply malloc_block; cbn; lia.
+        * apply write_block; cbn; lia.
+      + repeat rewrite sep_conj_perm_bottom. constructor; auto.
+        { intros [] (? & ? & ?). cbn in *.
+          rewrite Nat.sub_0_r in *. rewrite Nat.add_0_r in *.
+          split; split; auto.
+          - split; auto. symmetry. apply write_block.
+          - symmetry. apply separate_sep_conj_perm.
+            + apply malloc_write. cbn; lia.
+            + apply malloc_block; cbn; lia.
+            + apply write_block.
+        }
+        { intros [] [] (? & ? & ?). cbn in *.
+          rewrite Nat.sub_0_r in *. rewrite Nat.add_0_r in *. auto. }
+        { intros [] [] H. rewrite sep_conj_perm_assoc in H.
+          rewrite Nat.sub_0_r in *. rewrite Nat.add_0_r in *.
+          unfold post_malloc_perm. unfold guar. unfold guar_post_malloc.
+          unfold "**". unfold guar. unfold guar in H. unfold "**" in H. unfold guar in H.
+          replace (S size - 1) with size. 2: lia. apply H. (* TODO simplify this *)
+        }
+    - cbn. assert (Hn': (n <= size)%nat) by lia.
+      specialize (IHn (Vector.tl xs) Hn').
+      rewrite Nat.add_0_r in *.
+      destruct IHn as (? & ? & ? & ? & Hsep & Hlte).
+      destruct H as (? & ? & ? & ? & Hsep' & Hlte').
+      destruct H as (? & ? & ? & ? & Hsep'' & Hlte'').
+      (* destruct H0 as (? & (? & ?) & ?). subst. *)
+      (* destruct H1 as (? & (? & ?) & ?). subst. *)
+      exists (write_perm (b, size - S n) (VNum 0) ** x).
+      eexists. split; [| split; [| split]]; eauto.
+      2: {
+        symmetry. apply separate_sep_conj_perm.
+        2: symmetry; auto.
+        - symmetry. eapply separate_antimonotone. apply write_post_malloc_perm; auto.
+          etransitivity; eauto. apply lte_r_sep_conj_perm.
+        - symmetry. eapply separate_antimonotone. apply write_post_malloc_perm; auto.
+          etransitivity; eauto. apply lte_l_sep_conj_perm.
+      }
+      {
+        exists (write_perm (b, size - S n) (VNum 0) ** x1). eexists.
+        split; [| split; [| split]]. 2: apply H1.
+        3: { rewrite sep_conj_perm_assoc. apply sep_conj_perm_monotone; auto. reflexivity. }
+        2: {
+          symmetry. apply separate_sep_conj_perm.
+          2: symmetry; auto.
+          - symmetry. eapply separate_antimonotone. apply write_post_malloc_perm; auto.
+            etransitivity; eauto. etransitivity. 2: apply lte_l_sep_conj_perm.
+            etransitivity; eauto. apply lte_r_sep_conj_perm.
+          - symmetry. eapply separate_antimonotone. apply write_post_malloc_perm; auto.
+            etransitivity; eauto. etransitivity. 2: apply lte_l_sep_conj_perm.
+            etransitivity; eauto. apply lte_l_sep_conj_perm.
+        }
+        do 2 eexists. split; [| split; [| split]].
+        - eexists. split. exists (VNum 0). reflexivity.
+          eexists. exists bottom_perm. split; [| split; [| split]]; cbn; try reflexivity.
+          apply separate_bottom.
+        - assert (Heq : size - S n + 1 = size - n) by lia. rewrite Heq. clear Heq.
+          exists x3, x4. split; [| split]; eauto.
+          rewrite arr_offset in *. cbn in *.
+          assert (Heq : size - S n + 2 = size - n + 1) by lia. rewrite Heq. clear Heq. auto.
+        - rewrite sep_conj_perm_bottom.
+          eapply separate_antimonotone. apply write_post_malloc_perm; auto.
+          etransitivity; eauto. etransitivity. 2: apply lte_l_sep_conj_perm.
+          etransitivity; eauto. apply lte_l_sep_conj_perm.
+        - rewrite sep_conj_perm_bottom. reflexivity.
+      }
+      {
+        etransitivity. 2: apply post_malloc_perm_extend; auto.
+        rewrite sep_conj_perm_assoc. apply sep_conj_perm_monotone; auto. reflexivity.
+      }
+  Qed.
+
+  Lemma Malloc xi xs size :
+    xi :: eqp (S size) ▷ xs * malloc_Perms ⊢
+    malloc xi ⤳
+    Ret (Vector.const tt (S size), tt) :::
+    (arr (W, 0, S size, trueP)) ⋆ (blockPT (S size)) ∅ malloc_Perms.
+  Proof.
+    intros p si ss Hp Hpre. pstep. unfold malloc.
+    destruct Hp as (peq & pmalloc & Heq & Hpmalloc & Hsep & Hlte). cbn in Heq. subst.
+    destruct Hpmalloc as (? & (b & ?) & Hpmalloc); subst.
+    (* read step *)
+    rewritebisim @bind_trigger. econstructor; eauto; try reflexivity.
+    (* write step *)
+    rewritebisim @bind_trigger. unfold id. econstructor; eauto.
+    { apply Hlte in Hpre. destruct Hpre as (_ & Hpre & _).
+      apply Hpmalloc in Hpre. apply Hlte. constructor 1. right. apply Hpmalloc.
+      cbn in *. split.
+      - eexists. reflexivity.
+      - intros ptr Hb. split; rewrite lGetPut.
+        + unfold read, allocated. subst. rewrite nth_error_app_early; auto.
+        + unfold sizeof. subst. rewrite nth_error_app_early; auto.
+    }
+    (* return *)
+    { eapply sep_step_lte. etransitivity. 2: apply Hlte.
+      etransitivity. 2: apply lte_r_sep_conj_perm. apply Hpmalloc.
+      apply sep_step_malloc with (size := size).
+    }
+    { apply Hlte in Hpre. destruct Hpre as (_ & Hpre & Hlte').
+      apply Hpmalloc in Hpre. cbn in Hpre.
+      constructor.
+      - cbn. repeat rewrite lGetPut. split; [| split].
+        + rewrite last_length. lia.
+        + unfold sizeof. cbn.
+          rewrite nth_error_app_last; auto.
+        + intros. unfold read, allocated. cbn. rewrite nth_error_app_last; auto.
+          rewrite (Bool.reflect_iff _ _ (Nat.ltb_spec0 _ _)) in H. cbn in *. rewrite H. auto.
+      - unfold "∅", "⋆", ptApp.
+        setoid_rewrite Hpre.
+        replace 0 with (size - size) at 2. 2: lia.
+        apply post_malloc_perm_ok; auto.
+    }
+  Qed.
+
+  (** * Free *)
+
+  (* helper lemma for Free *)
+  Lemma combined_arr_guar {A} p parr b len n bytes (v : Vector.t A n) (si : Si) (ss : Ss)
+        (Hb : b < length (lget si))
+        (Hn: (n <= (S len))%nat)
+        (Hlte : parr <= p)
+        (Hblock: nth_error (lget si) b = Some (Some (LBlock (S len) bytes)))
+        (Hparr: parr ∈ VPtr (b, 0) :: arr (W, (S len) - n, n, trueP) ▷ v) :
+    let si' := lput si (replace_n (lget si) b (S len) bytes n) in
+    (forall ptr', b <> fst ptr' -> read (lget si) ptr' = read (lget si') ptr') ->
+    (forall ptr', sizeof (lget si) ptr' = sizeof (lget si') ptr') ->
+    length (lget si) = length (lget si') ->
+    guar p (si, ss) (si', ss).
+  Proof.
+    revert Hlte Hparr Hblock Hb Hn. revert b parr v. revert n.
+    induction n; intros.
+    - apply Hlte. subst si'. cbn in *.
+      rewrite replace_n_0; auto. rewrite lPutGet. reflexivity.
+    - destruct Hparr as (pptr & parr' & Hpptr & Hparr' & Hsep & Hlte').
+      etransitivity.
+      {
+        eapply IHn; try lia; try rewrite lGetPut.
+        2: { cbn in Hparr'. rewrite Nat.sub_succ_l. eauto. lia. }
+        all: auto.
+        - etransitivity; eauto. etransitivity; eauto. apply lte_r_sep_conj_perm.
+        - cbn. intros. pose proof @read_replace_n_neq; eauto.
+        - cbn. intros. pose proof sizeof_replace_n; eauto.
+        - apply replace_list_index_length; auto.
+      }
+      {
+        subst si'. cbn. apply Hlte. apply Hlte'. constructor 1. left.
+        destruct Hpptr as (val & (? & ?) & Hpptr); subst.
+        destruct Hpptr as (pwrite & p' & Hpwrite & _ & Hsep' & Hlte'').
+        apply Hlte''. constructor 1. left.
+        apply Hpwrite. cbn.
+        repeat rewrite lGetPut in *.
+        split; [| split; [| split]]; auto.
+        - eexists. rewrite lPutPut. reflexivity.
+        - intros. destruct (Nat.eq_dec b (fst ptr')).
+          2: { pose proof read_replace_n_neq. cbn in H3. repeat rewrite <- H3; auto. }
+          subst. destruct ptr' as [b o]. simpl in *.
+          assert (Hneq: len - n <> o).
+          { apply addr_neq_cases in H2. destruct H2; auto. }
+          unfold replace_n, read, allocated. simpl.
+          repeat rewrite nth_error_replace_list_index_eq; auto.
+          destruct (o <? S len) eqn:?; auto.
+          rewrite Bool.andb_true_l. simpl.
+          destruct (S len - n <=? o) eqn:?.
+          + pose proof Heqb1.
+            assert (Himpl: (S len - n <= o -> len - n <= o)%nat) by lia.
+            rewrite <- (Bool.reflect_iff _ _ (Nat.leb_spec0 _ _)) in H3. apply Himpl in H3.
+            rewrite (Bool.reflect_iff _ _ (Nat.leb_spec0 _ _)) in H3.
+            rewrite H3. simpl in Heqb1. rewrite Heqb1. auto.
+          + pose proof Heqb1.
+            simpl in Heqb1. rewrite Heqb1.
+            apply Nat.leb_gt in H3.
+            assert (len - n > o) by lia.
+            apply Compare_dec.leb_correct_conv in H4. rewrite H4. auto.
+        - intros. pose proof sizeof_replace_n. simpl in H2. rewrite <- H2; auto.
+        - unfold replace_n. erewrite <- replace_list_index_length; eauto.
+      }
+  Qed.
+
+  Lemma Free {A} xi len (xs : Vector.t A (S len) * unit) :
+    xi :: (arr (W, 0, (S len), trueP)) ⋆ (blockPT (S len)) ▷ xs ⊢
+       free xi ⤳
+       Ret tt :::
+       trueP.
+  Proof.
+    intros p si ss (parr & pblock & Hparr & Hpblock & Hsep & Hlte) Hpre.
+    pstep. unfold free. destruct xi as [| ptr]; try contradiction.
+    assert (Hoffset: snd ptr = 0).
+    { apply Hlte in Hpre. destruct Hpre as (_ & Hpre & _).
+      apply Hpblock in Hpre. simpl in Hpre. unfold sizeof in Hpre.
+      rewrite (Bool.reflect_iff _ _ (Nat.eqb_spec _ _)).
+      destruct (snd ptr =? 0); inversion Hpre; auto.
+    }
+    rewrite Hoffset. simpl.
+    (* read step *)
+    rewritebisim @bind_trigger. econstructor; auto; try reflexivity.
+    pose proof Hpre as Hpre'. apply Hlte in Hpre'.
+    destruct Hpre' as (Hprewrite & Hpreblock & Hsep').
+    apply Hpblock in Hpreblock. simpl in Hpreblock.
+    unfold sizeof in Hpreblock. rewrite Hoffset in Hpreblock. simpl in Hpreblock.
+    unfold memory in *.
+    destruct (nth_error (lget si) (fst ptr)) eqn:?; try solve [inversion Hpreblock].
+    destruct o; try solve [inversion Hpreblock].
+    destruct l. inversion Hpreblock; clear Hpreblock; subst.
+    (* write step *)
+    rewritebisim @bind_trigger. unfold id. econstructor; auto.
+    - apply Hlte. constructor 1. left.
+      assert (Hb: fst ptr < length (lget si)).
+      { apply nth_error_Some. intro. rewrite H in Heqo. inversion Heqo. }
+      erewrite replace_n_same.
+      eapply combined_arr_guar; eauto; try reflexivity; try rewrite lGetPut.
+      + destruct ptr. simpl in Hoffset. subst. rewrite Nat.sub_diag. apply Hparr.
+      + intros. erewrite read_replace_n_neq; eauto.
+      + intros. erewrite sizeof_replace_n; eauto.
+      + apply replace_list_index_length; auto.
+    - apply sep_step_lte'. apply bottom_perm_is_bottom.
+    - constructor; simpl; auto.
+  Qed.
+
+  (** * Reachability rules *)
+  Lemma ReflR {A} x rw o (T : @VPermType Si Ss A) :
+    x :: trueP ▷ tt ⊨ x :: reach_perm x rw o T ▷ nil.
+  Proof.
+    repeat intro. apply mu_fixed_point. reflexivity.
+  Qed.
+
+  Lemma TransR {A} x y z rw o (T : @VPermType Si Ss A) xs ys :
+    x :: reach_perm y rw o T ▷ xs * y :: reach_perm z rw o T ▷ ys ⊨
+                                     x :: reach_perm z rw o T ▷ (xs ++ ys).
+  Proof.
+    revert x.
+    induction xs.
+    - intros x p (p1 & p2 & Hp1 & Hp2 & Hsep & Hlte).
+      destruct Hp1 as (? & (U & HU & ?) & Hp1); subst.
+      apply HU in Hp1. simpl in Hp1. subst. eapply Perms_upwards_closed; eauto.
+      etransitivity; eauto. apply lte_r_sep_conj_perm.
+    - intros x p (px' & py & Hpx' & Hpy & Hsep & Hlte).
+      eapply mu_fixed_point in Hpx'.
+      destruct Hpx' as (pa & px & Hpa & Hpx & Hsep' & Hlte').
+      (* x must be a pointer *)
+      destruct x; try contradiction. destruct a0 as [b o'].
+      destruct Hpx as (? & (v & ?) & Hpx); subst.
+      destruct Hpx as (px'' & pv & Hpx'' & Hpv & Hsep'' & Hlte'').
+
+      apply mu_fixed_point.
+      simpl.
+      exists pa. exists (px'' ** (pv ** py)). split; [apply Hpa | split; [| split]].
+      2: {
+        apply separate_sep_conj_perm.
+        - eapply separate_antimonotone; eauto.
+          etransitivity; eauto. apply lte_l_sep_conj_perm.
+        - apply separate_sep_conj_perm.
+          + eapply separate_antimonotone; eauto.
+            etransitivity; eauto. apply lte_r_sep_conj_perm.
+          + symmetry. symmetry in Hsep. eapply separate_antimonotone; eauto.
+            etransitivity; eauto. apply lte_l_sep_conj_perm.
+          + symmetry in Hsep. eapply separate_antimonotone; eauto.
+            etransitivity; eauto. etransitivity. apply lte_r_sep_conj_perm.
+            apply sep_conj_perm_monotone. reflexivity.
+            etransitivity; eauto. apply lte_r_sep_conj_perm.
+        - symmetry. apply separate_sep_conj_perm.
+          + eapply separate_antimonotone; eauto. reflexivity.
+          + symmetry. symmetry in Hsep. eapply separate_antimonotone; eauto.
+            etransitivity; eauto. etransitivity. apply lte_r_sep_conj_perm.
+            apply sep_conj_perm_monotone. reflexivity.
+            etransitivity; eauto. apply lte_l_sep_conj_perm.
+          + symmetry in Hsep. eapply separate_antimonotone; eauto.
+            etransitivity; eauto. etransitivity. apply lte_r_sep_conj_perm.
+            apply sep_conj_perm_monotone. reflexivity.
+            etransitivity; eauto. apply lte_r_sep_conj_perm.
+      }
+      2: { repeat rewrite <- sep_conj_perm_assoc.
+           etransitivity; eauto.
+           eapply sep_conj_perm_monotone; intuition.
+           repeat rewrite sep_conj_perm_assoc.
+           etransitivity; eauto.
+           eapply sep_conj_perm_monotone; intuition.
+      }
+      eexists. split; [eexists; reflexivity |].
+      apply sep_conj_Perms_perm; [apply Hpx'' | |].
+      2: {
+        apply separate_sep_conj_perm; auto.
+        + symmetry. symmetry in Hsep. eapply separate_antimonotone; eauto.
+          etransitivity; eauto. etransitivity. apply lte_r_sep_conj_perm.
+          apply sep_conj_perm_monotone. reflexivity.
+          etransitivity; eauto. apply lte_l_sep_conj_perm.
+        + symmetry in Hsep. eapply separate_antimonotone; eauto.
+          etransitivity; eauto. etransitivity. apply lte_r_sep_conj_perm.
+          apply sep_conj_perm_monotone. reflexivity.
+          etransitivity; eauto. apply lte_r_sep_conj_perm.
+      }
+      cbn. exists (v :: reach_perm z rw o T ▷ (xs ++ ys)). split.
+      2: {
+        apply IHxs. apply sep_conj_Perms_perm; auto.
+        symmetry. symmetry in Hsep. eapply separate_antimonotone; eauto.
+        etransitivity; eauto. etransitivity. apply lte_r_sep_conj_perm.
+        apply sep_conj_perm_monotone. reflexivity.
+        etransitivity; eauto. apply lte_r_sep_conj_perm.
+      }
+      eexists; split; eauto.
+      repeat intro. eapply mu_fixed_point in H; auto.
+      Unshelve. all: apply reach_perm_proper.
+  Qed.
+
 End MemoryPerms.
+
+Notation "'arr' ( rw , o , l , T )" := (arr_perm rw o l T).
