src/PermTypeProofs.v
@@ -17,7 +17,6 @@ From Heapster Require Export
      Utils
      Permissions
      Memory
-     MemoryPerms
      SepStep
      Typing
      PermType.
@@ -41,1146 +40,274 @@ Import ITreeNotations.
 Local Open Scope itree_scope.
 (* end hide *)
 
-Context (Si Ss:Type).
-Context `{Lens Si memory}.
+Section Rules.
+  Context (Si Ss:Type).
 
-(** * Basic permission connective rules *)
+  (** * Basic permission connective rules *)
 
-Lemma Weak (A B : Type) P1 P2 (U1 U2 : PermType Si Ss A B) ts ti :
-  P1 ⊨ P2 ->
-  (forall xi xs, xi :: U2 ▷ xs ⊨ xi :: U1 ▷ xs) ->
-  P2 ⊢ ts ⤳ ti ::: U2 ->
-  P1 ⊢ ts ⤳ ti ::: U1.
-Proof.
-  intros. eapply typing_lte; eauto.
-Qed.
+  Lemma Weak (A B : Type) P1 P2 (U1 U2 : @PermType Si Ss A B) ts ti :
+    P1 ⊨ P2 ->
+    (forall xi xs, xi :: U2 ▷ xs ⊨ xi :: U1 ▷ xs) ->
+    P2 ⊢ ts ⤳ ti ::: U2 ->
+    P1 ⊢ ts ⤳ ti ::: U1.
+  Proof.
+    intros. eapply typing_lte; eauto.
+  Qed.
 
-Lemma ProdI (A1 A2 B1 B2 : Type) xi yi xs ys (T1 : PermType Si Ss A1 B1) (T2 : PermType Si Ss A2 B2) :
-  xi :: T1 ▷ xs * yi :: T2 ▷ ys ⊨ (xi, yi) :: T1 ⊗ T2 ▷ (xs, ys).
-Proof. reflexivity. Qed.
+  Lemma ProdI (A1 A2 B1 B2 : Type) xi yi xs ys (T1 : @PermType Si Ss A1 B1) (T2 : @PermType Si Ss A2 B2) :
+    xi :: T1 ▷ xs * yi :: T2 ▷ ys ⊨ (xi, yi) :: T1 ⊗ T2 ▷ (xs, ys).
+  Proof. reflexivity. Qed.
 
-Lemma ProdE (A1 A2 B1 B2 : Type) xi xs (T1 : PermType Si Ss A1 B1) (T2 : PermType Si Ss A2 B2) :
-  xi :: T1 ⊗ T2 ▷ xs ⊨ fst xi :: T1 ▷ fst xs * snd xi :: T2 ▷ snd xs.
-Proof. reflexivity. Qed.
+  Lemma ProdE (A1 A2 B1 B2 : Type) xi xs (T1 : @PermType Si Ss A1 B1) (T2 : @PermType Si Ss A2 B2) :
+    xi :: T1 ⊗ T2 ▷ xs ⊨ fst xi :: T1 ▷ fst xs * snd xi :: T2 ▷ snd xs.
+  Proof. reflexivity. Qed.
 
-Lemma SumI1 (A1 A2 B1 B2 : Type) (xi : A1) (xs : B1) (T1 : PermType Si Ss A1 B1) (T2 : PermType Si Ss A2 B2) :
-  xi :: T1 ▷ xs ⊨ inl xi :: T1 ⊕ T2 ▷ inl xs.
-Proof. reflexivity. Qed.
+  Lemma SumI1 (A1 A2 B1 B2 : Type) (xi : A1) (xs : B1) (T1 : @PermType Si Ss A1 B1) (T2 : @PermType Si Ss A2 B2) :
+    xi :: T1 ▷ xs ⊨ inl xi :: T1 ⊕ T2 ▷ inl xs.
+  Proof. reflexivity. Qed.
 
-Lemma SumI2 (A1 A2 B1 B2 : Type) (xi : A2) (xs : B2) (T1 : PermType Si Ss A1 B1) (T2 : PermType Si Ss A2 B2) :
-  xi :: T2 ▷ xs ⊨ inr xi :: T1 ⊕ T2 ▷ inr xs.
-Proof. reflexivity. Qed.
+  Lemma SumI2 (A1 A2 B1 B2 : Type) (xi : A2) (xs : B2) (T1 : @PermType Si Ss A1 B1) (T2 : @PermType Si Ss A2 B2) :
+    xi :: T2 ▷ xs ⊨ inr xi :: T1 ⊕ T2 ▷ inr xs.
+  Proof. reflexivity. Qed.
 
-Lemma SumE (A1 A2 B1 B2 R1 R2 : Type)
-      (xi : A1 + A2) (xs : B1 + B2) ti1 ti2 ts1 ts2
-      (T1 : PermType Si Ss A1 B1) (T2 : PermType Si Ss A2 B2) (P : Perms) (U : PermType Si Ss (A1 + A2) (B1 + B2)) :
-  (forall yi ys, P * yi :: T1 ▷ ys ⊢ ti1 yi ⤳ ts1 ys ::: U) ->
-  (forall yi ys, P * yi :: T2 ▷ ys ⊢ ti2 yi ⤳ ts2 ys ::: U) ->
-  P * xi :: T1 ⊕ T2 ▷ xs ⊢ sum_rect _ ti1 ti2 xi ⤳ sum_rect _ ts1 ts2 xs ::: U.
-Proof.
-  intros. simpl.
-  destruct xi, xs; simpl; auto;
-    rewrite sep_conj_Perms_commut; rewrite sep_conj_Perms_top_absorb; apply typing_top.
-Qed.
+  Lemma SumE (A1 A2 B1 B2 R1 R2 : Type)
+        (xi : A1 + A2) (xs : B1 + B2) ti1 ti2 ts1 ts2
+        (T1 : @PermType Si Ss A1 B1) (T2 : @PermType Si Ss A2 B2) (P : Perms) (U : @PermType Si Ss (A1 + A2) (B1 + B2)) :
+    (forall yi ys, P * yi :: T1 ▷ ys ⊢ ti1 yi ⤳ ts1 ys ::: U) ->
+    (forall yi ys, P * yi :: T2 ▷ ys ⊢ ti2 yi ⤳ ts2 ys ::: U) ->
+    P * xi :: T1 ⊕ T2 ▷ xs ⊢ sum_rect _ ti1 ti2 xi ⤳ sum_rect _ ts1 ts2 xs ::: U.
+  Proof.
+    intros. simpl.
+    destruct xi, xs; cbn; auto;
+      rewrite sep_conj_Perms_commut; rewrite sep_conj_Perms_top_absorb; apply typing_top.
+  Qed.
 
-Lemma StarI (A B1 B2 : Type) xi xs ys (T1 : PermType Si Ss A B1) (T2 : PermType Si Ss A B2) :
-  xi :: T1 ▷ xs * xi :: T2 ▷ ys ⊨ xi :: T1 ⋆ T2 ▷ (xs, ys).
-Proof. reflexivity. Qed.
+  Lemma StarI (A B1 B2 : Type) xi xs ys (T1 : @PermType Si Ss A B1) (T2 : @PermType Si Ss A B2) :
+    xi :: T1 ▷ xs * xi :: T2 ▷ ys ⊨ xi :: T1 ⋆ T2 ▷ (xs, ys).
+  Proof. reflexivity. Qed.
 
-Lemma StarE (A B1 B2 : Type) xi xs (T1 : PermType Si Ss A B1) (T2 : PermType Si Ss A B2) :
-  xi :: T1 ⋆ T2 ▷ xs ⊨ xi :: T1 ▷ fst xs * xi :: T2 ▷ snd xs.
-Proof. reflexivity. Qed.
+  Lemma StarE (A B1 B2 : Type) xi xs (T1 : @PermType Si Ss A B1) (T2 : @PermType Si Ss A B2) :
+    xi :: T1 ⋆ T2 ▷ xs ⊨ xi :: T1 ▷ fst xs * xi :: T2 ▷ snd xs.
+  Proof. reflexivity. Qed.
 
-Lemma PermsI (A B : Type) (P : Perms) xi xs (T : PermType Si Ss A B) :
-  xi :: T ▷ xs * P ⊨ xi :: T ∅ P ▷ xs.
-Proof. reflexivity. Qed.
+  Lemma PermsI (A B : Type) (P : Perms) xi xs (T : @PermType Si Ss A B) :
+    xi :: T ▷ xs * P ⊨ xi :: T ∅ P ▷ xs.
+  Proof. reflexivity. Qed.
 
-Lemma PermsE (A B : Type) (P : Perms) xi xs (T : PermType Si Ss A B) :
-  xi :: T ∅ P ▷ xs ⊨ xi :: T ▷ xs * P.
-Proof. reflexivity. Qed.
+  Lemma PermsE (A B : Type) (P : Perms) xi xs (T : @PermType Si Ss A B) :
+    xi :: T ∅ P ▷ xs ⊨ xi :: T ▷ xs * P.
+  Proof. reflexivity. Qed.
 
-Lemma Frame (A B : Type) (P1 P2 : Perms) ti ts (T : PermType Si Ss A B) :
-  P1 ⊢ ti ⤳ ts ::: T ->
-  P1 * P2 ⊢ ti ⤳ ts ::: T ∅ P2.
-Proof. apply typing_frame. Qed.
+  Lemma Frame (A B : Type) (P1 P2 : Perms) ti ts (T : @PermType Si Ss A B) :
+    P1 ⊢ ti ⤳ ts ::: T ->
+    P1 * P2 ⊢ ti ⤳ ts ::: T ∅ P2.
+  Proof. apply typing_frame. Qed.
 
-Lemma OrI1 (A B1 B2 : Type) xi xs (T1 : PermType Si Ss A B1) (T2 : PermType Si Ss A B2) :
-  xi :: T1 ▷ xs ⊨ xi :: or _ _ T1 T2 ▷ inl xs.
-Proof. reflexivity. Qed.
+  Lemma OrI1 (A B1 B2 : Type) xi xs (T1 : @PermType Si Ss A B1) (T2 : @PermType Si Ss A B2) :
+    xi :: T1 ▷ xs ⊨ xi :: or T1 T2 ▷ inl xs.
+  Proof. reflexivity. Qed.
 
-Lemma OrI2 (A B1 B2 : Type) xi xs (T1 : PermType Si Ss A B1) (T2 : PermType Si Ss A B2) :
-  xi :: T2 ▷ xs ⊨ xi :: or _ _ T1 T2 ▷ inr xs.
-Proof. reflexivity. Qed.
+  Lemma OrI2 (A B1 B2 : Type) xi xs (T1 : @PermType Si Ss A B1) (T2 : @PermType Si Ss A B2) :
+    xi :: T2 ▷ xs ⊨ xi :: or T1 T2 ▷ inr xs.
+  Proof. reflexivity. Qed.
 
-Lemma OrE (A B1 B2 C1 C2 D : Type)
-      (xi : A) (xs : B1 + B2) ti ts1 ts2
-      (T1 : PermType Si Ss A B1) (T2 : PermType Si Ss A B2) (P : Perms) (U : PermType Si Ss D (C1 + C2)) :
-  (forall ys, P * xi :: T1 ▷ ys ⊢ ti ⤳ ts1 ys ::: U) ->
-  (forall ys, P * xi :: T2 ▷ ys ⊢ ti ⤳ ts2 ys ::: U) ->
-  P * xi :: or _ _ T1 T2 ▷ xs ⊢ ti ⤳ sum_rect _ ts1 ts2 xs ::: U.
-Proof.
-  intros. destruct xs; simpl; auto.
-Qed.
+  Lemma OrE (A B1 B2 C1 C2 D : Type)
+        (xi : A) (xs : B1 + B2) ti ts1 ts2
+        (T1 : @PermType Si Ss A B1) (T2 : @PermType Si Ss A B2) (P : Perms) (U : @PermType Si Ss D (C1 + C2)) :
+    (forall ys, P * xi :: T1 ▷ ys ⊢ ti ⤳ ts1 ys ::: U) ->
+    (forall ys, P * xi :: T2 ▷ ys ⊢ ti ⤳ ts2 ys ::: U) ->
+    P * xi :: or T1 T2 ▷ xs ⊢ ti ⤳ sum_rect _ ts1 ts2 xs ::: U.
+  Proof.
+    intros. destruct xs; cbn; auto.
+  Qed.
 
-Lemma TrueI (A : Type) P (xi : A) :
-  P ⊨ P * xi :: trueP Si Ss ▷ tt.
-Proof.
-  simpl. rewrite sep_conj_Perms_commut. rewrite sep_conj_Perms_bottom_identity. reflexivity.
-Qed.
+  Lemma TrueI (A : Type) (P : @Perms (Si * Ss)) (xi : A) :
+    P ⊨ P * xi :: trueP ▷ tt.
+  Proof.
+    rewrite sep_conj_Perms_commut. rewrite sep_conj_Perms_bottom_identity. reflexivity.
+  Qed.
 
-Lemma ExI (A B : Type) (C : B -> Type) (xi : A) (ys : B) (xs : C ys) (F : forall (b : B), PermType Si Ss A (C b)) :
-  xi :: F ys ▷ xs ⊨ xi :: ex (z oftype B) (F z) ▷ existT (fun b : B => C b) ys xs.
-Proof. reflexivity. Qed.
+  Lemma ExI (A B : Type) (C : B -> Type) (xi : A) (ys : B) (xs : C ys)
+        (F : forall (b : B), @PermType Si Ss A (C b)) :
+    xi :: F ys ▷ xs ⊨ xi :: ex (z oftype B) (F z) ▷ existT (fun b : B => C b) ys xs.
+  Proof. reflexivity. Qed.
 
-Lemma ExE (A B : Type) (C : B -> Type) (xi : A) (xs : sigT (fun b : B => C b)) (F : forall (b : B), PermType Si Ss A (C b)) :
-  xi :: ex (z oftype B) (F z) ▷ xs ⊨ xi :: F (projT1 xs) ▷ (projT2 xs).
-Proof. reflexivity. Qed.
+  Lemma ExE (A B : Type) (C : B -> Type) (xi : A) (xs : sigT (fun b : B => C b))
+        (F : forall (b : B), @PermType Si Ss A (C b)) :
+    xi :: ex (z oftype B) (F z) ▷ xs ⊨ xi :: F (projT1 xs) ▷ (projT2 xs).
+  Proof. reflexivity. Qed.
 
-(** * Equality rules *)
+  (** * Equality rules *)
 
-Lemma EqRefl A P (xi : A) :
-  P ⊨ P * xi :: eqp Si Ss xi ▷ tt.
-Proof.
-  repeat intro.
-  exists p, bottom_perm. split; [| split; [| split]]; cbn; eauto.
-  - apply separate_bottom.
-  - rewrite sep_conj_perm_bottom. reflexivity.
-Qed.
-
-Lemma EqSym (A : Type) (xi yi : A) :
-  xi :: eqp Si Ss yi ▷ tt ⊨ yi :: eqp _ _ xi ▷ tt.
-Proof.
-  repeat intro; simpl in *; subst; reflexivity.
-Qed.
-
-Lemma EqTrans (A : Type) (xi yi zi : A) :
-   xi :: eqp _ _ yi ▷ tt * yi :: eqp _ _ zi ▷ tt ⊨ xi :: eqp Si Ss zi ▷ tt.
-Proof.
-  repeat intro. destruct H0 as (? & ? & ? & ? & ?). simpl in *; subst. reflexivity.
-Qed.
-
-Lemma EqCtx (A B : Type) (xi yi : A) (f : A -> B) :
-  xi :: eqp _ _ yi ▷ tt ⊨ f xi :: eqp Si Ss (f yi) ▷ tt.
-Proof.
-  repeat intro. simpl in *. congruence.
-Qed.
-
-Lemma EqDup (A : Type) (xi yi : A) :
-  xi :: eqp _ _ yi ▷ tt ⊨ xi :: eqp Si Ss yi ▷ tt * xi :: eqp _ _ yi ▷ tt.
-Proof.
-  repeat intro. cbn in *. subst. exists bottom_perm, bottom_perm.
-  split; [| split; [| split]]; auto.
-  - apply separate_bottom.
-  - rewrite sep_conj_perm_bottom. apply bottom_perm_is_bottom.
-Qed.
-
-Lemma Cast (A B : Type) (P : PermType Si Ss A B) xi yi xs ys :
-  xi :: eqp _ _ yi ▷ xs * yi :: P ▷ ys ⊨ xi :: P ▷ ys.
-Proof.
-  repeat intro. destruct H0 as (e & p' & Heq & Hp & Hsep & Hlte).
-  simpl in Heq. subst.
-  eapply Perms_upwards_closed; eauto. etransitivity. apply lte_r_sep_conj_perm. eauto.
-Qed.
-
-(** * Instruction rules *)
-(** Name conflicts with ITree Ret. *)
-Lemma Ret_ (A B : Type) xi xs (T : PermType Si Ss A B) :
-  xi :: T ▷ xs ⊢ Ret xi ⤳ Ret xs ::: T.
-Proof.
-  repeat intro. pstep. constructor; auto.
-Qed.
-
-Lemma Bind (A B C D : Type) P ti ts fi fs (T : PermType Si Ss A B) (U : PermType Si Ss C D) :
-  P ⊢ ti ⤳ ts ::: T ->
-  (forall xi xs, xi :: T ▷ xs ⊢ fi xi ⤳ fs xs ::: U) ->
-  P ⊢ ITree.bind ti fi ⤳ ITree.bind ts fs ::: U.
-Proof.
-  intros. eapply typing_bind; eauto.
-Qed.
-
-Lemma GetNum xi yi :
-  xi :: eqp Si Ss (VNum yi) ▷ tt ⊢ getNum xi ⤳ Ret tt ::: eqp _ _ yi.
-Proof.
-  repeat intro. simpl in *. subst. simpl. pstep. constructor; auto. reflexivity.
-Qed.
-
-Lemma Iter (A B C D : Type) (T : PermType Si Ss C D) xi xs fi fs (U : PermType Si Ss A B) :
-  (forall yi ys, yi :: T ▷ ys ⊢ fi yi ⤳ fs ys ::: T ⊕ U) ->
-  xi :: T ▷ xs ⊢ iter fi xi ⤳ iter fs xs ::: U.
-Proof.
-  revert xi xs fi fs U. pcofix CIH. intros.
-  do 2 rewritebisim @unfold_iter_ktree.
-  eapply sbuter_bind; eauto.
-  - apply H1; auto.
-  - simpl. intros. destruct r1, r2; try contradiction.
-    + repeat intro. pstep. constructor 5; eauto.
-    + pstep. constructor; auto.
-Qed.
-
-Lemma If (A B : Type) P ti1 ti2 ts1 ts2 (xi yi : bool) xs (U : PermType Si Ss A B) :
-  P ⊢ ti1 ⤳ ts1 ::: U ->
-  P ⊢ ti2 ⤳ ts2 ::: U ->
-  P * xi :: eqp _ _ yi ▷ xs ⊢ if xi then ti1 else ti2 ⤳ if yi then ts1 else ts2 ::: U.
-Proof.
-  repeat intro. destruct H2 as (p' & q & Hp' & ? & Hsep & Hlte); cbn in *; subst.
-  destruct xi.
-  - apply H0; auto. eapply Perms_upwards_closed; eauto.
-    etransitivity; eauto. apply lte_l_sep_conj_perm.
-  - apply H1; auto. eapply Perms_upwards_closed; eauto.
-    etransitivity; eauto. apply lte_l_sep_conj_perm.
-Qed.
-
-Lemma Err (A B : Type) P (U : PermType Si Ss A B) t :
-  P ⊢ t ⤳ throw tt ::: U.
-Proof.
-  repeat intro. pstep. constructor.
-Qed.
-
-(** * Example 1 *)
-
-Definition ex1i xi : itree (sceE Si) Value :=
-  x <- getNum xi;;
-  Ret (VNum (Init.Nat.mul 5 x)).
-
-Definition ex1s (xs : sigT (fun _ : nat => unit)) : itree (sceE Ss) (sigT (fun _ : nat => unit)) :=
-  Ret tt;;
-  Ret (existT _ (Init.Nat.mul 5 (projT1 xs)) tt).
-
-Definition IsNat : VPermType Si Ss (sigT (fun _ : nat => unit)) :=
-  ex (n oftype nat) eqp Si Ss (VNum n).
-
-Lemma ex1_typing xi xs :
-  xi :: IsNat ▷ xs ⊢ ex1i xi ⤳ ex1s xs ::: IsNat.
-Proof.
-  (* ExE *)
-  unfold IsNat. eapply Weak; [eapply ExE | reflexivity |].
-  (* Bind *)
-  unfold ex1s, ex1i. eapply Bind.
-  (* GetNum *)
-  apply GetNum.
-  (* EqCtx *)
-  intros yi []. clear xi.
-  eapply Weak; [apply EqCtx with (f := fun x => VNum (Init.Nat.mul 5 x)) | reflexivity |].
-  (* ExI *)
-  eapply Weak; [apply ExI with (F := fun n : nat => eqp Si Ss (VNum n)) | reflexivity |]; fold IsNat.
-  (* Ret *)
-  apply Ret_.
-Qed.
-
-(** * Pointer rules *)
-
-Lemma PtrI A xi yi xs ys rw o (T : VPermType Si Ss A) :
-  xi :: ptr _ _ (rw, o, eqp Si Ss yi) ▷ xs * yi :: T ▷ ys ⊨ xi :: ptr _ _ (rw, o, T) ▷ ys.
-Proof.
-  destruct xi; simpl.
-  - rewrite sep_conj_Perms_top_absorb. reflexivity.
-  - repeat intro. destruct a. rename p into p'.
-    destruct H0 as (p & t & (P & (v & ?) & Hp) & Hp' & Hsep & Hlte). subst.
-    destruct Hp as (? & ? & ? & ? & Hsep' & Hlte'). cbn in *. subst.
-    eexists. split; [exists v; reflexivity |].
-    eapply Perms_upwards_closed; eauto.
-    do 2 eexists. split; [| split; [| split]]; eauto.
-    + symmetry. symmetry in Hsep. eapply separate_antimonotone; eauto.
-      etransitivity; eauto. apply lte_l_sep_conj_perm.
-    + apply sep_conj_perm_monotone; intuition.
-      etransitivity; eauto. apply lte_l_sep_conj_perm.
-Qed.
-
-Lemma PtrE A B C (P : Perms) rw o (T : VPermType Si Ss A) (xi : Value) xs ti ts (U : PermType Si Ss B C) :
-  (forall yi, P * xi :: ptr _ _ (rw, o, eqp Si Ss yi) ▷ tt * yi :: T ▷ xs ⊢ ti ⤳ ts ::: U) ->
-  P * xi :: ptr _ _ (rw, o, T) ▷ xs ⊢ ti ⤳ ts ::: U.
-Proof.
-  repeat intro. rename p into p''. destruct H1 as (p & p' & Hp & Hptr & Hsep & Hlte).
-  destruct xi; [contradiction | destruct a].
-  destruct Hptr as (? & (? & ?) & ?). subst.
-  destruct H3 as (pptr & pt & Hptr & Hpt & Hsep' & Hlte').
-  eapply H0; eauto. exists (p ** pptr), pt.
-  split; [| split; [| split]]; eauto.
-  - do 2 eexists. split; [| split; [| split]]. eauto. 3: reflexivity.
-    + eexists. split; eauto. do 2 eexists.
-      split; [| split; [| split]]. eauto. reflexivity. 2: apply sep_conj_perm_bottom'.
-      apply separate_bottom.
-    + eapply separate_antimonotone; eauto. etransitivity; eauto. apply lte_l_sep_conj_perm.
-  - symmetry. symmetry in Hsep'. apply separate_sep_conj_perm; auto.
-    + symmetry. eapply separate_antimonotone; eauto. etransitivity; eauto.
-      apply lte_r_sep_conj_perm.
-    + symmetry. eapply separate_antimonotone; eauto. etransitivity; eauto.
-      apply lte_l_sep_conj_perm.
-  - etransitivity; eauto. rewrite sep_conj_perm_assoc.
-    apply sep_conj_perm_monotone; auto; reflexivity.
-Qed.
-
-(* TODO: move to other file *)
-Lemma read_separate Ss ptr ptr' v v' :
-  (read_perm ptr v : @perm (Si * Ss)) ⊥ read_perm ptr' v'.
-Proof.
-  split; intros; auto; destruct x, y; cbn in *; subst; reflexivity.
-Qed.
-
-Lemma ReadDup o xi yi :
-  xi :: ptr _ _ (R, o, eqp _ _ yi) ▷ tt ⊨
-  xi :: ptr _ _ (R, o, eqp Si Ss yi) ▷ tt * xi :: ptr _ _ (R, o, eqp _ _ yi) ▷ tt.
-Proof.
-  repeat intro. simpl in *. destruct xi; [contradiction |].
-  destruct a as [b o']. unfold offset in *.
-  destruct H0 as (? & (v & ?) & ?). subst.
-  exists (read_perm (b, o' + o) v), (read_perm (b, o' + o) v).
-  destruct H1 as (pread & peq & Hpread & Hpeq & Hsep & Hlte).
-  simpl in Hpread, Hpeq. subst.
-  assert (read_perm (b, o' + o) v ∈ ptr_Perms _ _ R (VPtr (b, o' + o)) tt (eqp Si Ss v)).
-  {
-    eexists. split; eauto. simpl in *. exists (read_perm (b, o' + o) v), bottom_perm.
-    split; [| split; [| split]]. 2: reflexivity.
-    - split; intros; auto.
+  Lemma EqRefl A (P : @Perms (Si * Ss)) (xi : A) :
+    P ⊨ P * xi :: eqp xi ▷ tt.
+  Proof.
+    repeat intro.
+    exists p, bottom_perm. split; [| split; [| split]]; cbn; eauto.
     - apply separate_bottom.
     - rewrite sep_conj_perm_bottom. reflexivity.
-  }
-  split; [| split; [| split]]; auto.
-  apply read_separate.
-  constructor; intros; eauto.
-  - split; [| split]; auto. 1, 2: apply Hpread; apply Hlte; auto.
-    apply read_separate.
-  - split; apply Hpread; apply Hlte; auto.
-  - apply Hlte. constructor. left. apply Hpread. induction H1; auto.
-    + destruct H1; auto.
-    + etransitivity; eauto.
-Qed.
+  Qed.
 
-Lemma PtrOff A xi xs rw o1 o2 (T : VPermType Si Ss A) :
-  o1 >= o2 ->
-  xi :: ptr _ _ (rw, o1, T) ▷ xs ⊨ offset xi o2 :: ptr _ _ (rw, o1 - o2, T) ▷ xs.
-Proof.
-  destruct xi; [reflexivity | destruct a].
-  intros. simpl. rewrite <- Nat.add_assoc.
-  rewrite (Nat.add_comm o2 _). rewrite Nat.sub_add; auto.
-  reflexivity.
-Qed.
-Lemma PtrOff' A xi xs rw o1 o2 (T : VPermType Si Ss A) :
-  o1 >= o2 ->
-  offset xi o2 :: ptr _ _ (rw, o1 - o2, T) ▷ xs ⊨ xi :: ptr _ _ (rw, o1, T) ▷ xs.
-Proof.
-  destruct xi; [reflexivity | destruct a].
-  intros. cbn. rewrite <- Nat.add_assoc.
-  rewrite (Nat.add_comm o2 _). rewrite Nat.sub_add; auto.
-  reflexivity.
-Qed.
+  Lemma EqSym (A : Type) (xi yi : A) :
+    xi :: @eqp Si Ss _ yi ▷ tt ⊨ yi :: eqp xi ▷ tt.
+  Proof.
+    repeat intro; cbn in *; subst; reflexivity.
+  Qed.
 
-Lemma Load xi yi xs rw :
-  xi :: ptr _ _ (rw, 0, eqp Si Ss yi) ▷ xs ⊢
-  load xi ⤳
-  Ret tt :::
-  eqp _ _ yi ∅ xi :: ptr _ _ (rw, 0, eqp _ _ yi) ▷ xs.
-Proof.
-  repeat intro. pstep. unfold load. rewritebisim @bind_trigger.
-  econstructor; eauto; try reflexivity.
-  destruct xi as [? | [b o]]; try contradiction.
-  cbn in H0. unfold ptr_Perms in H0.
-  destruct H0 as (? & (v & ?) & ?); subst.
-  destruct H2 as (? & ? & ? & ? & Hsep & Hlte). cbn in H0, H2. subst.
-  assert (read (lget c1) (b, o) = Some v).
-  {
-    apply Hlte in H1. destruct H1 as (? & _).
-    rewrite Nat.add_0_r in H0. apply H0 in H1. destruct rw; auto.
-  }
-  rewrite H2. constructor; auto.
-  (* TODO: these exists are kind of weird *)
-  cbn. exists bottom_perm, x. split; [| split; [| split]]; auto.
-  - cbn. eexists. split; eauto.
-    cbn. exists x, bottom_perm. split; [| split; [| split]]; eauto.
-    apply separate_bottom.
-    rewrite sep_conj_perm_bottom. reflexivity.
-  - symmetry. apply separate_bottom.
-  - rewrite sep_conj_perm_commut. rewrite sep_conj_perm_bottom.
-    etransitivity; eauto. apply lte_l_sep_conj_perm.
-Qed.
+  Lemma EqTrans (A : Type) (xi yi zi : A) :
+    xi :: @eqp Si Ss _ yi ▷ tt * yi :: eqp zi ▷ tt ⊨ xi :: eqp zi ▷ tt.
+  Proof.
+    repeat intro. destruct H as (? & ? & ? & ? & ? & ?). cbn in *; subst. reflexivity.
+  Qed.
 
-Lemma Store A xi yi xs (P : VPermType Si Ss A) :
-  xi :: ptr _ _ (W, 0, P) ▷ xs ⊢
-  store xi yi ⤳
-  Ret tt :::
-  (trueP Si Ss) ∅ xi :: ptr _ _ (W, 0, eqp _ _ yi) ▷ tt.
-Proof.
-  repeat intro. pstep. unfold store. destruct xi as [| [b o]]; try contradiction.
-  rewritebisim @bind_trigger.
-  rename p into p'. rename H1 into Hpre.
-  destruct H0 as (? & (v & ?) & Hwrite); subst.
-  destruct Hwrite as (pw & p & Hwritelte & Hp & Hsep & Hlte).
-  rewrite Nat.add_0_r in Hwritelte.
-  assert (exists val, read (lget c1) (b, o) = Some val).
-  {
-    apply Hlte in Hpre. destruct Hpre as (Hpre & _).
-    apply Hwritelte in Hpre. eexists.
-    symmetry. apply Hpre.
-  }
-  destruct H0 as (val & Hread). eapply (read_success_write _ _ _ yi) in Hread.
-  destruct Hread as (c' & Hwrite).
-  assert (Hguar : guar p' (c1, c2) ((lput c1 c'), c2)).
-  {
-    apply Hlte. constructor 1. left. apply Hwritelte. simpl.
-    split; [| split]; rewrite lGetPut.
-    + eapply write_success_read_neq; eauto.
-    + eapply write_success_sizeof; eauto.
-    + eapply write_success_length; eauto.
-  }
-  econstructor; eauto.
-  3: {
-    rewrite Hwrite. constructor; eauto.
-    2: { simpl. exists bottom_perm. eexists. split; [| split; [| split]]; auto.
-         - eexists. split; eauto. simpl. eexists. exists bottom_perm.
-           split; [| split; [| split]]; eauto; try reflexivity.
-           apply separate_bottom.
-         - symmetry. apply separate_bottom.
-         - rewrite sep_conj_perm_bottom. rewrite sep_conj_perm_commut.
-           rewrite sep_conj_perm_bottom. reflexivity.
-    }
-    rewrite Nat.add_0_r. symmetry. eapply write_success_read_eq; rewrite lGetPut; eauto.
-  }
-  - rewrite Hwrite. auto.
-  - rewrite Nat.add_0_r. eapply sep_step_lte; eauto.
-    etransitivity.
-    + eapply sep_step_lte; [| reflexivity]. apply lte_l_sep_conj_perm.
-    + simpl in *. eapply sep_step_lte; eauto. intros ? []. constructor; auto.
-Qed.
+  Lemma EqCtx (A B : Type) (xi yi : A) (f : A -> B) :
+    xi :: eqp yi ▷ tt ⊨ f xi :: @eqp Si Ss _ (f yi) ▷ tt.
+  Proof.
+    repeat intro. congruence.
+  Qed.
 
-Lemma IsNull1 A xi xs rw o (P : VPermType Si Ss A) :
-  xi :: ptr _ _ (rw, o, P) ▷ xs ⊢
-  isNull xi ⤳
-  Ret tt :::
-  eqp _ _ false ∅ xi :: ptr _ _ (rw, o, P) ▷ xs.
-Proof.
-  repeat intro. pstep. unfold isNull. destruct xi; [contradiction |].
-  destruct a as [b o']. simpl. constructor; auto.
-  cbn. exists bottom_perm, p. split; [| split; [| split]]; eauto.
-  - symmetry. apply separate_bottom.
-  - rewrite sep_conj_perm_commut. rewrite sep_conj_perm_bottom. reflexivity.
-Qed.
+  Lemma EqDup (A : Type) (xi yi : A) :
+    xi :: @eqp Si Ss _ yi ▷ tt ⊨ xi :: eqp yi ▷ tt * xi :: eqp yi ▷ tt.
+  Proof.
+    repeat intro. cbn in *. subst. exists bottom_perm, bottom_perm.
+    split; [| split; [| split]]; auto.
+    - apply separate_bottom.
+    - rewrite sep_conj_perm_bottom. apply bottom_perm_is_bottom.
+  Qed.
 
-Lemma IsNull2 xi:
-  xi :: eqp Si Ss (VNum 0) ▷ tt ⊢
-  isNull xi ⤳
-  Ret tt :::
-  eqp _ _ true.
-Proof.
-  repeat intro. pstep. cbn in *. subst. constructor; cbn; auto.
-Qed.
+  Lemma Cast (A B : Type) (P : @PermType Si Ss A B) xi yi xs ys :
+    xi :: eqp yi ▷ xs * yi :: P ▷ ys ⊨ xi :: P ▷ ys.
+  Proof.
+    repeat intro. destruct H as (e & p' & Heq & Hp & Hsep & Hlte).
+    cbn in Heq. subst.
+    eapply Perms_upwards_closed; eauto. etransitivity. apply lte_r_sep_conj_perm. eauto.
+  Qed.
 
-(** * Example 2 *)
+  (** * Instruction rules *)
+  (** Name conflicts with ITree Ret. *)
+  Lemma Ret_ (A B : Type) xi xs (T : @PermType Si Ss A B) :
+    xi :: T ▷ xs ⊢ Ret xi ⤳ Ret xs ::: T.
+  Proof.
+    repeat intro. pstep. constructor; auto.
+  Qed.
 
-Definition ex2i xi yi : itree (sceE Si) Si :=
-  x <- load xi;;
-  store yi x.
+  Lemma Bind (A B C D : Type) P ti ts fi fs (T : @PermType Si Ss A B) (U : @PermType Si Ss C D) :
+    P ⊢ ti ⤳ ts ::: T ->
+    (forall xi xs, xi :: T ▷ xs ⊢ fi xi ⤳ fs xs ::: U) ->
+    P ⊢ ITree.bind ti fi ⤳ ITree.bind ts fs ::: U.
+  Proof.
+    intros. eapply typing_bind; eauto.
+  Qed.
 
-Definition ex2s : itree (sceE Ss) unit :=
-  Ret tt ;;
-  Ret tt.
+  Lemma GetNum xi yi :
+    xi :: @eqp Si Ss _ (VNum yi) ▷ tt ⊢ getNum xi ⤳ Ret tt ::: eqp yi.
+  Proof.
+    repeat intro. cbn in *. subst. cbn. pstep. constructor; auto. reflexivity.
+  Qed.
 
-Lemma ex2_typing A (xi yi : Value) xs (T : VPermType Si Ss A) :
-  xi :: ptr _ _ (R, 0, T) ▷ xs * yi :: ptr Si Ss (W, 0, trueP _ _) ▷ tt ⊢
-  ex2i xi yi ⤳
-  ex2s :::
-  (trueP _ _) ∅ yi :: ptr _ _ (W, 0, T) ▷ xs ∅ xi :: ptr _ _ (R, 0, trueP _ _) ▷ tt.
-Proof.
-  (* PtrE *)
+  Lemma Iter (A B C D : Type) (T : @PermType Si Ss C D) xi xs fi fs (U : @PermType Si Ss A B) :
+    (forall yi ys, yi :: T ▷ ys ⊢ fi yi ⤳ fs ys ::: T ⊕ U) ->
+    xi :: T ▷ xs ⊢ iter fi xi ⤳ iter fs xs ::: U.
+  Proof.
+    revert xi xs fi fs U. pcofix CIH. intros.
+    do 2 rewritebisim @unfold_iter_ktree.
+    eapply sbuter_bind; eauto.
+    - apply H0; auto.
+    - cbn. intros. destruct r1, r2; try contradiction.
+      + repeat intro. pstep. constructor 5; eauto.
+      + pstep. constructor; auto.
+  Qed.
 
-  rewrite sep_conj_Perms_commut.
-  eapply PtrE; eauto; intros zi.
-  (* Bind *)
-  eapply Bind.
-  (* L: Frame and Load *)
-  apply Frame. rewrite sep_conj_Perms_commut. apply Frame. apply Load.
-  (* Weak *)
-  intros wi [].
-  eapply Weak with (P2 := yi :: ptr _ _ (W, 0, trueP _ _) ▷ tt *
-                          wi :: T ▷ xs *
-                          xi :: ptr _ _ (R, 0, trueP _ _) ▷ tt)
-                   (U2 := trueP _ _ ∅
-                          yi :: ptr _ _ (W, 0, eqp _ _ wi) ▷ tt ∅
-                          wi :: T ▷ xs ∅
-                          xi :: ptr _ _ (R, 0, trueP _ _) ▷ tt).
-  (* Input type *)
-  - etransitivity.
-    (* PermsE *)
-    {
-      etransitivity; [apply PermsE |]. rewrite sep_conj_Perms_commut.
-      eapply sep_conj_Perms_monotone; [reflexivity |]. (* frame *)
-      etransitivity; [| apply PermsE]. rewrite sep_conj_Perms_commut.
-      eapply sep_conj_Perms_monotone; [reflexivity |]. (* frame *)
-      etransitivity; [| apply PermsE]. rewrite sep_conj_Perms_commut. reflexivity.
-    }
-    rewrite (sep_conj_Perms_commut (zi :: T ▷ xs) _).
-    repeat rewrite <- sep_conj_Perms_assoc.
-    apply sep_conj_Perms_monotone; [reflexivity |].
-    rewrite sep_conj_Perms_commut.
-    eapply sep_conj_Perms_monotone.
-    (* Weakening the content type *)
-    + etransitivity; [apply PtrI | apply TrueI].
-    (* Cast *)
-    + apply Cast.
-  (* Output type *)
-  - intros ? [].
-    etransitivity; [apply PermsE |].
-    etransitivity; [| apply PermsI].
-    eapply sep_conj_Perms_monotone; [| reflexivity]. (* frame *)
-    etransitivity; [| apply PermsE].
-    etransitivity; [apply PermsI |].
-    etransitivity.
-    2: {
-      eapply sep_conj_Perms_monotone; [| reflexivity]. (* frame *)
-      apply PermsE.
-    }
-    rewrite <- sep_conj_Perms_assoc.
-    eapply sep_conj_Perms_monotone; [reflexivity |]. (* frame *)
-    (* PtrI *)
-    apply PtrI.
-    (* Frame and Store *)
-  - apply Frame. apply Frame. apply Store.
-Qed.
+  Lemma If (A B : Type) P ti1 ti2 ts1 ts2 (xi yi : bool) xs (U : @PermType Si Ss A B) :
+    P ⊢ ti1 ⤳ ts1 ::: U ->
+    P ⊢ ti2 ⤳ ts2 ::: U ->
+    P * xi :: eqp yi ▷ xs ⊢ if xi then ti1 else ti2 ⤳ if yi then ts1 else ts2 ::: U.
+  Proof.
+    repeat intro. destruct H1 as (p' & q & Hp' & ? & Hsep & Hlte); cbn in *; subst.
+    destruct xi.
+    - apply H; auto. eapply Perms_upwards_closed; eauto.
+      etransitivity; eauto. apply lte_l_sep_conj_perm.
+    - apply H0; auto. eapply Perms_upwards_closed; eauto.
+      etransitivity; eauto. apply lte_l_sep_conj_perm.
+  Qed.
 
-(** * Array rules *)
+  Lemma Err (A B : Type) P (U : @PermType Si Ss A B) t :
+    P ⊢ t ⤳ throw tt ::: U.
+  Proof.
+    repeat intro. pstep. constructor.
+  Qed.
 
-(** Some helper lemmas? TODO *)
-Fixpoint split_leq {A} l1 (v:Vector.t A l1) :
-  forall l2, le l2 l1 -> (Vector.t A l2 * Vector.t A (l1 - l2)).
-Proof.
-  destruct v; intros; destruct l2.
-  - split; apply Vector.nil.
-  - elimtype False; inversion H0.
-  - split; [ apply Vector.nil | apply Vector.cons; assumption ].
-  - edestruct (split_leq _ n v l2) as [v1 v2].
-    + apply le_S_n; assumption.
-    + split; [ apply Vector.cons; assumption | assumption ].
-Defined.
+  (** * Example 1 *)
 
-Fixpoint append_leq {A} l1 l2 (l: le l2 l1)
-         (v1:Vector.t A l2) (v2:Vector.t A (l1 - l2)) : Vector.t A l1.
-Proof.
-  revert l2 l v1 v2. destruct l1; intros.
-  - constructor.
-  - destruct l2.
-    + apply v2.
-    + constructor; [ apply (Vector.hd v1) | ]. apply (append_leq _ l1 l2).
-      * apply le_S_n; assumption.
-      * apply (Vector.tl v1).
-      * apply v2.
-Defined.
+  Definition ex1i xi : itree (sceE Si) Value :=
+    x <- getNum xi;;
+    Ret (VNum (Init.Nat.mul 5 x)).
 
-Arguments append_leq {A} !l1.
-Arguments split_leq {A} l1 !v.
+  Definition ex1s (xs : sigT (fun _ : nat => unit)) : itree (sceE Ss) (sigT (fun _ : nat => unit)) :=
+    Ret tt;;
+    Ret (existT _ (Init.Nat.mul 5 (projT1 xs)) tt).
 
-Lemma split_leq_append_leq A l1 v l2 (l: le l2 l1) :
-  @append_leq A l1 l2 l (fst (split_leq l1 v l2 l)) (snd (split_leq l1 v l2 l)) = v.
-Proof.
-  revert l2 l; induction v; intros.
-  - cbn. reflexivity.
-  - destruct l2.
-    + cbn. reflexivity.
-    + cbn.
-      rewrite (surjective_pairing (split_leq n v l2 (le_S_n l2 n l))). simpl.
-      rewrite IHv. reflexivity.
-Qed.
+  Definition IsNat : @VPermType Si Ss (sigT (fun _ : nat => unit)) :=
+    ex (n oftype nat) eqp (VNum n).
 
-Definition trySplit {A l1 R S} (v : Vector.t A l1) l2 (f : Vector.t A l2 -> Vector.t A (l1 - l2) -> itree (sceE S) R) : itree (sceE S) R.
-  destruct (le_lt_dec l2 l1).
-  - exact (f (fst (split_leq l1 v l2 l)) (snd (split_leq l1 v l2 l))).
-  - exact (throw tt).
-Defined.
+  Lemma ex1_typing xi xs :
+    xi :: IsNat ▷ xs ⊢ ex1i xi ⤳ ex1s xs ::: IsNat.
+  Proof.
+    (* ExE *)
+    unfold IsNat. eapply Weak; [eapply ExE | reflexivity |].
+    (* Bind *)
+    unfold ex1s, ex1i. eapply Bind.
+    (* GetNum *)
+    apply GetNum.
+    (* EqCtx *)
+    intros yi []. clear xi.
+    eapply Weak; [apply EqCtx with (f := fun x => VNum (Init.Nat.mul 5 x)) | reflexivity |].
+    (* ExI *)
+    eapply Weak; [apply ExI with (F := fun n : nat => eqp (VNum n)) | reflexivity |]; fold IsNat.
+    (* Ret *)
+    apply Ret_.
+  Qed.
 
-Lemma ArrCombine_eq A xi rw o l1 l2 (l:le l2 l1) xs1 xs2 (P : VPermType Si Ss A) :
-  eq_Perms (xi :: arr (rw, o, l1, P) ▷ append_leq l1 l2 l xs1 xs2)
-           (xi :: arr (rw, o, l2, P) ▷ xs1 * xi :: arr (rw, o + l2, l1 - l2, P) ▷ xs2).
-Proof.
-  revert o l2 l xs1 xs2; induction l1; intros.
-  - inversion l. subst. simpl. rewrite sep_conj_Perms_bottom_identity. reflexivity.
-  - destruct l2.
-    + simpl. rewrite sep_conj_Perms_bottom_identity.
-      rewrite Nat.add_0_r. reflexivity.
-    + simpl. rewrite (IHl1 (S o) l2).
-      simpl. rewrite Nat.add_succ_r.
-      rewrite sep_conj_Perms_assoc.
-      reflexivity.
-Qed.
+  (** * Recursive and reachability rules *)
 
-Lemma ArrSplit A R1 R2 P l1 l2 xi xs rw o (T : VPermType Si Ss A) U (ti : itree (sceE Si) R1) (fs : _ -> _ -> itree (sceE Ss) R2) :
-  (forall xs1 xs2, P *
-              xi :: arr (rw, o, l2, T) ▷ xs1 *
-              xi :: arr (rw, o + l2, l1 - l2, T) ▷ xs2 ⊢
-              ti ⤳ fs xs1 xs2 ::: U) ->
-  P * xi :: arr (rw, o, l1, T) ▷ xs ⊢ ti ⤳ trySplit xs l2 fs ::: U.
-Proof.
-  intros. unfold trySplit. destruct (le_lt_dec l2 l1).
-  - rewrite <- (split_leq_append_leq _ l1 xs l2 l).
-    rewrite ArrCombine_eq. repeat rewrite split_leq_append_leq.
-    rewrite sep_conj_Perms_assoc.
-    apply H0.
-  - apply Err.
-Qed.
+  Lemma MuFold A G X `{FixedPoint G X} (F : @PermType Si Ss A X -> @PermType Si Ss A (G X))
+        {prp : Proper (lte_PermType ==> lte_PermType) F}
+        xi xs :
+    xi :: F (mu F) ▷ xs ⊨ xi :: mu F ▷ foldFP xs.
+  Proof.
+    (* FIXME: why can't we just rewrite with mu_fixed_point here? *)
+    eapply Proper_eq_Perms_lte_Perms; [ | reflexivity | ].
+    - apply Proper_eq_PermType_ptApp; [ apply mu_fixed_point | | ]; reflexivity.
+    - simpl. rewrite foldUnfold. reflexivity.
+  Qed.
 
-Lemma vector_tl_append A n m (v1 : Vector.t A (S n)) (v2 : Vector.t A m) :
-  Vector.tl (Vector.append v1 v2) = Vector.append (Vector.tl v1) v2.
-Proof.
-  revert v1. revert n. apply Vector.caseS. intros; auto.
-Qed.
+  Lemma MuUnfold A G X `{FixedPoint G X} (F : @PermType Si Ss A X -> @PermType Si Ss A (G X))
+        {prp : Proper (lte_PermType ==> lte_PermType) F}
+        xi xs :
+    xi :: mu F ▷ xs ⊨ xi :: F (mu F) ▷ unfoldFP xs.
+  Proof.
+    eapply Proper_eq_Perms_lte_Perms; [ reflexivity | | ].
+    - apply Proper_eq_PermType_ptApp; [ apply mu_fixed_point | | ]; reflexivity.
+    - simpl. reflexivity.
+  Qed.
 
-Lemma vector_hd_append A n m (v1 : Vector.t A (S n)) (v2 : Vector.t A m) :
-  Vector.hd (Vector.append v1 v2) = Vector.hd v1.
-Proof.
-  revert v1. revert n. apply Vector.caseS. intros; auto.
-Qed.
+  (* Program Definition list_reach_perm r rw A (T : VPermType Si Ss A) : VPermType Si Ss (list A) := *)
+  (*   @mu _ _ _ (mu_list A) _ (fixed_point_list _) *)
+  (*       (fun U => or _ _ (eqp Si Ss r) ((ptr _ _ (rw, 0, T)) ⋆ (ptr _ _ (rw, 1, U)))) _. *)
+  (* Next Obligation. *)
+  (*   repeat intro. simpl. induction b; simpl in *; auto. *)
+  (*   destruct H0 as (? & ? & ? & ? & ?). exists x0, x1. split; [| split]; auto. *)
+  (*   clear H0. unfold ptr_Perms in *. destruct (offset a 1); auto. *)
+  (*   destruct H1. destruct H0. destruct H0. subst. destruct H1 as (? & ? & ? & ? & ?). *)
+  (*   eexists. split; eauto. do 2 eexists. split; eauto. split; eauto. apply H. auto. *)
+  (* Qed. *)
 
-Lemma ArrCombine A xi rw o l1 l2 xs1 xs2 (P : VPermType Si Ss A) :
-  xi :: arr (rw, o, l1, P) ▷ xs1 * xi :: arr (rw, o + l1, l2, P) ▷ xs2 ⊨
-  xi :: arr (rw, o, l1 + l2, P) ▷ Vector.append xs1 xs2 .
-Proof.
-  repeat intro. destruct H0 as (p1 & p2 & Hp1 & Hp2 & Hsep & Hlte).
-  revert Hp1 Hp2. revert o xi l2 xs2. revert Hsep Hlte. revert p p1 p2. induction l1; intros.
-  - rewrite Nat.add_0_r in Hp2. cbn in *. revert xs1. apply Vector.case0. simpl.
-    eapply Perms_upwards_closed; eauto. etransitivity; [apply lte_r_sep_conj_perm |]; eauto.
-  - cbn. destruct Hp1 as (? & ? & ? & ? & Hsep' & Hlte').
-    do 2 eexists. split; [| split; [| split]].
-    + rewrite vector_hd_append. apply H0.
-    + rewrite vector_tl_append. eapply IHl1. 2: reflexivity.
-      2: { eapply Perms_upwards_closed; eauto. reflexivity. }
-      2: { cbn. rewrite <- plus_n_Sm in Hp2. eauto. }
-      symmetry. symmetry in Hsep. eapply separate_antimonotone; eauto.
-      etransitivity; eauto. apply lte_r_sep_conj_perm.
-    + apply separate_sep_conj_perm; auto.
-      * symmetry. symmetry in Hsep. eapply separate_antimonotone; eauto.
-        etransitivity; eauto. apply lte_l_sep_conj_perm.
-      * symmetry in Hsep. eapply separate_antimonotone; eauto.
-        etransitivity; eauto. apply lte_r_sep_conj_perm.
-    + rewrite <- sep_conj_perm_assoc. etransitivity; eauto.
-      apply sep_conj_perm_monotone; eauto; reflexivity.
-Qed.
-
-Lemma ArrPtr A xi xs rw o (P : VPermType Si Ss A) :
-  xi :: arr (rw, o, 1, P) ▷ xs ⊨ xi :: ptr _ _ (rw, o, P) ▷ Vector.hd xs.
-Proof.
-  cbn. rewrite sep_conj_Perms_commut. rewrite sep_conj_Perms_bottom_identity. reflexivity.
-Qed.
-
-Lemma PtrArr A xi xs rw o (P : VPermType Si Ss A) :
-  xi :: ptr _ _ (rw, o, P) ▷ xs ⊨ xi :: arr (rw, o, 1, P) ▷ vsingle xs.
-Proof.
-  cbn. rewrite sep_conj_Perms_commut. rewrite sep_conj_Perms_bottom_identity. reflexivity.
-Qed.
-
-
-Lemma arr_offset {A} ptr rw o l (T : VPermType Si Ss A) (v : Vector.t A l) :
-  VPtr ptr :: arr (rw, o, l, T) ▷ v ≡ offset (VPtr ptr) o :: arr (rw, 0, l, T) ▷ v.
-Proof.
-  revert ptr o. induction l; intros; try reflexivity.
-  split.
-  - simpl. apply sep_conj_Perms_monotone.
-    + destruct ptr. simpl. rewrite Nat.add_0_r. reflexivity.
-    + destruct ptr. rewrite (IHl _ _ 1). simpl.
-      specialize (IHl (Vector.tl v) (n, n0) (o + 1)). simpl in IHl.
-      rewrite Nat.add_assoc in IHl. rewrite Nat.add_1_r in IHl. apply IHl.
-  - simpl. apply sep_conj_Perms_monotone.
-    + destruct ptr. simpl. rewrite Nat.add_0_r. reflexivity.
-    + destruct ptr. rewrite (IHl _ _ 1). simpl.
-      specialize (IHl (Vector.tl v) (n, n0) (o + 1)). simpl in IHl.
-      rewrite Nat.add_assoc in IHl. rewrite Nat.add_1_r in IHl. apply IHl.
-Qed.
-
-(** helper lemmas for Malloc *)
-Fixpoint rely_post_malloc n b size x y : Prop :=
-  match n with
-  | 0 => rely (block_perm size (b, 0) ** malloc_perm (b + 1)) x y
-  | S n => rely (@write_perm Si Ss _ (b, size - S n) (VNum 0)) x y /\
-          rely_post_malloc n b size x y
-  end.
-Lemma PO_rely_post_malloc n b size :
-  PreOrder (rely_post_malloc n b size).
-Proof.
-  constructor.
-  - intros []; induction n; simpl; auto.
-  - intros [] [] [] ? ?. induction n.
-    + split; [| split]; try solve [etransitivity; [apply H0 | apply H1]].
-      intros; split; (etransitivity; [apply H0 | apply H1]); auto.
-    + split; try solve [etransitivity; [apply H0 | apply H1]].
-      apply IHn; [apply H0 | apply H1].
-Qed.
-
-Fixpoint guar_post_malloc n b size x y : Prop :=
-  match n with
-  | 0 => guar (block_perm size (b, 0) ** malloc_perm (b + 1)) x y
-  | S n => clos_trans _ (fun x y =>
-                          guar (@write_perm Si Ss _ (b, size - S n) (VNum 0)) x y \/
-                          guar_post_malloc n b size x y) x y
-  end.
-#[local] Instance PO_guar_post_malloc n b size :
-  PreOrder (guar_post_malloc n b size).
-Proof.
-  constructor.
-  - intros []. induction n; simpl; intuition.
-  - intros [] [] [] ? ?.
-    destruct n; econstructor 2; eauto.
-Qed.
-
-Definition pre_post_malloc n b size : Si * Ss -> Prop :=
-  fun '(x, _) =>
-    b + 1 = length (lget x) /\
-    Some size = sizeof (lget x) (b, 0) /\
-    forall o, o < size -> (size - n <= o)%nat -> Some (VNum 0) = read (lget x) (b, o).
-Lemma pre_respects_post_malloc n b size :
-  forall x y, rely_post_malloc (S n) b size x y -> (* we need the fact that n > 0 here *)
-         pre_post_malloc (S n) b size x ->
-         pre_post_malloc (S n) b size y.
-Proof.
-  intros [] [] Hrely (Hlen & Hsizeof & Hread).
-  simpl in *.
-  induction n; simpl in *.
-  - destruct Hrely as (Hread' & Hsizeof' & Hlen' & Hptr).
-    split; [rewrite <- Hlen' | split; [rewrite <- Hsizeof' |]]; auto.
-    intros. assert (o = size - 1) by lia. subst.
-    rewrite <- Hread'. auto.
-  - destruct Hrely as (Hread' & Head'' & Hrely). split; [| split].
-    + apply IHn; auto. intros. apply Hread; auto. lia.
-    + apply IHn; auto. intros. apply Hread; auto. lia.
-    + intros. assert (size - S (S n) = o \/ (size - S n <= o)%nat) by lia.
-      destruct H2.
-      * subst. rewrite <- Hread'. auto.
-      * apply IHn; auto. intros. apply Hread; auto. lia.
-Qed.
-
-(** The intermediate permission for Malloc. *)
-(** [n] is the number of unfoldings to do for the rely/guar. [size] is the size of the block.
-    when we use this [n = size], but we need them separate to do induction on [n] *)
-Program Definition post_malloc_perm n b size : @perm (Si * Ss) :=
-  {|
-  rely := rely_post_malloc (S n) b (S size);
-  rely_PO := PO_rely_post_malloc (S n) b (S size);
-  guar := guar_post_malloc (S n) b (S size);
-  guar_PO := PO_guar_post_malloc (S n) b (S size);
-  pre := pre_post_malloc (S n) b (S size);
-  pre_respects := pre_respects_post_malloc n b (S size); (* S is applied inside this defn *)
-  |}.
-
-Lemma guar_malloc_post_malloc n b size x y :
-  guar_post_malloc n b (S size) x y -> guar (malloc_perm b) x y.
-Proof.
-  revert x y. induction n; intros.
-  - induction H0; try solve [etransitivity; eauto]. destruct H0.
-    + destruct x, y. simpl in *. subst; auto.
-    + destruct x, y. split; apply H0; lia.
-  - induction H0; auto.
-    + destruct H0.
-      * destruct x, y. destruct H0 as (? & ? & ?). split; auto.
-        apply H0. destruct ptr. intro. inversion H4. simpl in *. lia.
-      * apply IHn; auto.
-    + etransitivity; eauto.
-Qed.
-
-Lemma rely_malloc_post_malloc n b size x y :
-  rely (malloc_perm b) x y -> rely_post_malloc n b (S size) x y.
-Proof.
-  destruct x, y. induction n; intros.
-  - destruct H0 as (Hlen & Hptr).
-    split; [| split]; simpl; auto.
-    + apply Hptr; simpl; auto.
-    + intros. apply Hptr; lia.
-  - split; auto. simpl in *. apply H0. auto.
-Qed.
-
-Lemma sep_step_malloc n b size : sep_step (malloc_perm b)
-                                          (post_malloc_perm n b size).
-Proof.
-  apply sep_step_rg.
-  - apply guar_malloc_post_malloc.
-  - apply rely_malloc_post_malloc.
-Qed.
-
-Lemma write_post_malloc_perm m n size b
-      (Hsize : (m <= size)%nat)
-      (Hm : m > n):
-  write_perm (b, size - m) (VNum 0) ⊥ post_malloc_perm n b size.
-Proof.
-  constructor; auto; intros.
-  - revert H0. revert x y. induction n; intros.
-    + induction H0; try solve [etransitivity; eauto].
-      destruct H0; [| induction H0; try solve [etransitivity; eauto]; destruct H0].
-      * eapply write_write_sep; eauto. intro. inversion H1. lia.
-      * eapply write_block; eauto.
-      * eapply malloc_write; eauto. rewrite Nat.add_1_r in H0. auto.
-    + induction H0; try solve [etransitivity; eauto].
-      destruct H0. 2: apply IHn; auto; lia.
-      eapply write_write_sep; eauto. intro. inversion H1. lia.
-  - revert H0. revert x y. induction n; intros.
-    + destruct x, y. split; [| split; [| split; [| split]]]; simpl in *; try apply H0.
-      * intro. inversion H1. lia.
-      * destruct ptr. intro. simpl in *. inversion H2. lia.
-    + destruct x, y. simpl in H0. split; [| split]; simpl; try apply H0.
-      * intro. inversion H1. lia.
-      * intro. inversion H1. lia.
-      * apply IHn. lia. auto.
-Qed.
-
-Lemma post_malloc_perm_extend b size n (Hn : (S n <= size)%nat) :
-  write_perm (b, size - S n) (VNum 0) ** post_malloc_perm n b size <=
-  post_malloc_perm (S n) b size.
-Proof.
-  constructor; auto.
-  simpl in *; auto. intros [] H. destruct H as (Hlen & Hsizeof & Hread).
-  split; [| split; [split; [| split] |]]; auto; try solve [intros; apply Hread; lia].
-  apply write_post_malloc_perm; auto.
-Qed.
-
-Lemma post_malloc_perm_ok {A} n b size (xs : Vector.t A (S n))
-  (Hn : (n <= size)%nat) :
-  post_malloc_perm n b size (* the perm applies S to n and size inside *) ∈
-  VPtr (b, size - n) :: arr_perm Si Ss W 0 (S n) (trueP Si Ss) ▷ xs *
-  singleton_Perms (block_perm (S size) (b, 0)) *
-  malloc_Perms.
-Proof.
-  cbn. induction n.
-  - cbn. do 2 eexists. split; [| split; [| split]].
-    + do 2 eexists. split; [| split; [| split]]; try reflexivity.
-      * eexists. exists bottom_perm. split; [| split; [| split]]; auto. 3: reflexivity.
-        2: apply separate_bottom.
-        eexists. split; [exists (VNum 0); reflexivity |].
-        eexists. exists bottom_perm. split; [| split; [| split]]; cbn; try reflexivity.
-        apply separate_bottom.
-      * do 2 rewrite sep_conj_perm_bottom. symmetry. apply write_block.
-    + eexists. split; [exists (b + 1); reflexivity | cbn; reflexivity].
-    + do 2 rewrite sep_conj_perm_bottom. symmetry. apply separate_sep_conj_perm.
-      * apply malloc_write; cbn; lia.
-      * apply malloc_block; cbn; lia.
-      * apply write_block; cbn; lia.
-    + repeat rewrite sep_conj_perm_bottom. constructor; auto.
-      { intros [] (? & ? & ?). simpl in *.
-        rewrite Nat.sub_0_r in *. rewrite Nat.add_0_r in *.
-        split; split; auto.
-        - split; auto. symmetry. apply write_block.
-        - symmetry. apply separate_sep_conj_perm.
-          + apply malloc_write. simpl. lia.
-          + apply malloc_block; simpl; lia.
-          + apply write_block.
-      }
-      { intros [] [] (? & ? & ?). simpl in *.
-        rewrite Nat.sub_0_r in *. rewrite Nat.add_0_r in *. auto. }
-      { intros [] [] H. rewrite sep_conj_perm_assoc in H.
-        rewrite Nat.sub_0_r in *. rewrite Nat.add_0_r in *.
-        unfold post_malloc_perm. unfold guar. unfold guar_post_malloc.
-        unfold "**". unfold guar. unfold guar in H. unfold "**" in H. unfold guar in H.
-        replace (S size - 1) with size. 2: lia. apply H. (* TODO simplify this *)
-      }
-  - cbn. assert (Hn': (n <= size)%nat) by lia.
-    specialize (IHn (Vector.tl xs) Hn').
-    rewrite Nat.add_0_r in *.
-    destruct IHn as (? & ? & ? & ? & Hsep & Hlte).
-    destruct H0 as (? & ? & ? & ? & Hsep' & Hlte').
-    destruct H0 as (? & ? & ? & ? & Hsep'' & Hlte'').
-    (* destruct H0 as (? & (? & ?) & ?). subst. *)
-    (* destruct H1 as (? & (? & ?) & ?). subst. *)
-    exists (write_perm (b, size - S n) (VNum 0) ** x).
-    eexists. split; [| split; [| split]]; eauto.
-    2: {
-      symmetry. apply separate_sep_conj_perm.
-      2: symmetry; auto.
-      - symmetry. eapply separate_antimonotone. apply write_post_malloc_perm; auto.
-        etransitivity; eauto. apply lte_r_sep_conj_perm.
-      - symmetry. eapply separate_antimonotone. apply write_post_malloc_perm; auto.
-        etransitivity; eauto. apply lte_l_sep_conj_perm.
-    }
-    {
-      exists (write_perm (b, size - S n) (VNum 0) ** x1). eexists.
-      split; [| split; [| split]]. 2: apply H2.
-      3: { rewrite sep_conj_perm_assoc. apply sep_conj_perm_monotone; auto. reflexivity. }
-      2: {
-      symmetry. apply separate_sep_conj_perm.
-      2: symmetry; auto.
-      - symmetry. eapply separate_antimonotone. apply write_post_malloc_perm; auto.
-        etransitivity; eauto. etransitivity. 2: apply lte_l_sep_conj_perm.
-        etransitivity; eauto. apply lte_r_sep_conj_perm.
-      - symmetry. eapply separate_antimonotone. apply write_post_malloc_perm; auto.
-        etransitivity; eauto. etransitivity. 2: apply lte_l_sep_conj_perm.
-        etransitivity; eauto. apply lte_l_sep_conj_perm.
-      }
-      do 2 eexists. split; [| split; [| split]].
-      - eexists. split. exists (VNum 0). reflexivity.
-        eexists. exists bottom_perm. split; [| split; [| split]]; cbn; try reflexivity.
-        apply separate_bottom.
-      - assert (Heq : size - S n + 1 = size - n) by lia. rewrite Heq. clear Heq.
-        exists x3, x4. split; [| split]; eauto.
-        rewrite arr_offset in *. simpl in *.
-        assert (Heq : size - S n + 2 = size - n + 1) by lia. rewrite Heq. clear Heq. auto.
-      - rewrite sep_conj_perm_bottom.
-        eapply separate_antimonotone. apply write_post_malloc_perm; auto.
-        etransitivity; eauto. etransitivity. 2: apply lte_l_sep_conj_perm.
-        etransitivity; eauto. apply lte_l_sep_conj_perm.
-      - rewrite sep_conj_perm_bottom. reflexivity.
-    }
-    {
-      etransitivity. 2: apply post_malloc_perm_extend; auto.
-      rewrite sep_conj_perm_assoc. apply sep_conj_perm_monotone; auto. reflexivity.
-    }
-Qed.
-
-Lemma Malloc xi xs size :
-  xi :: eqp _ _ (S size) ▷ xs * malloc_Perms ⊢
-  malloc xi ⤳
-  Ret (Vector.const tt (S size), tt) :::
-  (arr (W, 0, S size, trueP Si Ss)) ⋆ (blockPT _ _ (S size)) ∅ malloc_Perms.
-Proof.
-  intros p si ss Hp Hpre. pstep. unfold malloc.
-  destruct Hp as (peq & pmalloc & Heq & Hpmalloc & Hsep & Hlte). simpl in Heq. subst.
-  destruct Hpmalloc as (? & (b & ?) & Hpmalloc); subst.
-  (* read step *)
-  rewritebisim @bind_trigger. econstructor; eauto; try reflexivity.
-  (* write step *)
-  rewritebisim @bind_trigger. unfold id. econstructor; eauto.
-  { apply Hlte in Hpre. destruct Hpre as (_ & Hpre & _).
-    apply Hpmalloc in Hpre. apply Hlte. constructor 1. right. apply Hpmalloc.
-    simpl in *.
-    intros ptr Hb. split; rewrite lGetPut.
-    - unfold read, allocated. subst. rewrite nth_error_app_early; auto.
-    - unfold sizeof. subst. rewrite nth_error_app_early; auto.
-  }
-  (* return *)
-  { eapply sep_step_lte. etransitivity. 2: apply Hlte.
-    etransitivity. 2: apply lte_r_sep_conj_perm. apply Hpmalloc.
-    apply sep_step_malloc with (size := size).
-  }
-  { apply Hlte in Hpre. destruct Hpre as (_ & Hpre & Hlte').
-    apply Hpmalloc in Hpre. simpl in Hpre.
-    constructor.
-    - simpl. split; [| split]; rewrite lGetPut.
-      + rewrite last_length. lia.
-      + unfold sizeof. simpl.
-        rewrite nth_error_app_last; auto.
-      + intros. unfold read, allocated. simpl. rewrite nth_error_app_last; auto.
-        rewrite (Bool.reflect_iff _ _ (Nat.ltb_spec0 _ _)) in H0. rewrite H0. auto.
-    - unfold "∅", "⋆", ptApp.
-      setoid_rewrite Hpre.
-      replace 0 with (size - size) at 2. 2: lia.
-      apply post_malloc_perm_ok; auto.
-  }
-Qed.
-
-(* helper lemma for Free *)
-Lemma combined_arr_guar {A} p parr b len n bytes (v : Vector.t A n) (si : Si) (ss : Ss)
-      (Hb : b < length (lget si))
-      (Hn: (n <= (S len))%nat)
-      (Hlte : parr <= p)
-      (Hblock: nth_error (lget si) b = Some (Some (LBlock (S len) bytes)))
-      (Hparr: parr ∈ VPtr (b, 0) :: arr (W, (S len) - n, n, trueP Si Ss) ▷ v) :
-  let si' := lput si (replace_n (lget si) b (S len) bytes n) in
-  (forall ptr', b <> fst ptr' -> read (lget si) ptr' = read (lget si') ptr') ->
-  (forall ptr', sizeof (lget si) ptr' = sizeof (lget si') ptr') ->
-  length (lget si) = length (lget si') ->
-  guar p (si, ss) (si', ss).
-Proof.
-  revert Hlte Hparr Hblock Hb Hn. revert b parr v. revert n.
-  induction n; intros.
-  - apply Hlte. subst si'. simpl in *.
-    rewrite replace_n_0; auto. rewrite lPutGet. reflexivity.
-  - destruct Hparr as (pptr & parr' & Hpptr & Hparr' & Hsep & Hlte').
-    etransitivity.
-    {
-      eapply IHn; try lia; try rewrite lGetPut.
-      2: { simpl in Hparr'. rewrite Nat.sub_succ_l. eauto. lia. }
-      - etransitivity; eauto. etransitivity; eauto. apply lte_r_sep_conj_perm.
-      - simpl. auto.
-      - lia.
-      - simpl. intros. pose proof @read_replace_n_neq; eauto.
-      - simpl. intros. pose proof sizeof_replace_n; eauto.
-      - apply replace_list_index_length; auto.
-    }
-    {
-      subst si'. simpl. apply Hlte. apply Hlte'. constructor 1. left.
-      destruct Hpptr as (val & (? & ?) & Hpptr); subst.
-      destruct Hpptr as (pwrite & p' & Hpwrite & _ & Hsep' & Hlte'').
-      apply Hlte''. constructor 1. left.
-      apply Hpwrite. simpl.
-      split; [| split]; auto; repeat rewrite lGetPut in *.
-      - intros. destruct (Nat.eq_dec b (fst ptr')).
-        2: { pose proof read_replace_n_neq. simpl in H3. repeat rewrite <- H4; auto. }
-        subst. destruct ptr' as [b o]. simpl in *.
-        assert (Hneq: len - n <> o).
-        { apply addr_neq_cases in H3. destruct H3; auto. }
-        unfold replace_n, read, allocated. simpl.
-        repeat rewrite nth_error_replace_list_index_eq; auto.
-        destruct (o <? S len) eqn:?; auto.
-        rewrite Bool.andb_true_l. simpl.
-        destruct (S len - n <=? o) eqn:?.
-        + pose proof Heqb1.
-          assert (Himpl: (S len - n <= o -> len - n <= o)%nat) by lia.
-          rewrite <- (Bool.reflect_iff _ _ (Nat.leb_spec0 _ _)) in H4. apply Himpl in H4.
-          rewrite (Bool.reflect_iff _ _ (Nat.leb_spec0 _ _)) in H4.
-          rewrite H4. simpl in Heqb1. rewrite Heqb1. auto.
-        + pose proof Heqb1.
-          simpl in Heqb1. rewrite Heqb1.
-          apply Nat.leb_gt in H4.
-          assert (len - n > o) by lia.
-          apply leb_correct_conv in H5. rewrite H5. auto.
-      - intros. pose proof sizeof_replace_n. simpl in H3. rewrite <- H3; auto.
-      - unfold replace_n. erewrite <- replace_list_index_length; eauto.
-    }
-Qed.
-
-Lemma Free {A} xi len (xs : Vector.t A (S len) * unit) :
-  xi :: (arr (W, 0, (S len), trueP Si Ss)) ⋆ (blockPT _ _ (S len)) ▷ xs ⊢
-  free xi ⤳
-  Ret tt :::
-  trueP _ _.
-Proof.
-  intros p si ss (parr & pblock & Hparr & Hpblock & Hsep & Hlte) Hpre.
-  pstep. unfold free. destruct xi as [| ptr]; try contradiction.
-  assert (Hoffset: snd ptr = 0).
-  { apply Hlte in Hpre. destruct Hpre as (_ & Hpre & _).
-    apply Hpblock in Hpre. simpl in Hpre. unfold sizeof in Hpre.
-    rewrite (Bool.reflect_iff _ _ (Nat.eqb_spec _ _)).
-    destruct (snd ptr =? 0); inversion Hpre; auto.
-  }
-  rewrite Hoffset. simpl.
-  (* read step *)
-  rewritebisim @bind_trigger. econstructor; auto; try reflexivity.
-  pose proof Hpre as Hpre'. apply Hlte in Hpre'.
-  destruct Hpre' as (Hprewrite & Hpreblock & Hsep').
-  apply Hpblock in Hpreblock. simpl in Hpreblock.
-  unfold sizeof in Hpreblock. rewrite Hoffset in Hpreblock. simpl in Hpreblock.
-  unfold memory in *.
-  destruct (nth_error (lget si) (fst ptr)) eqn:?; try solve [inversion Hpreblock].
-  destruct o; try solve [inversion Hpreblock].
-  destruct l. inversion Hpreblock; clear Hpreblock; subst.
-  (* write step *)
-  rewritebisim @bind_trigger. unfold id. econstructor; auto.
-  - apply Hlte. constructor 1. left.
-    assert (Hb: fst ptr < length (lget si)).
-    { apply nth_error_Some. intro. rewrite H0 in Heqo. inversion Heqo. }
-    erewrite replace_n_same.
-    eapply combined_arr_guar; eauto; try reflexivity; try rewrite lGetPut.
-    + destruct ptr. simpl in Hoffset. subst. rewrite Nat.sub_diag. apply Hparr.
-    + intros. erewrite read_replace_n_neq; eauto.
-    + intros. erewrite sizeof_replace_n; eauto.
-    + apply replace_list_index_length; auto.
-  - apply sep_step_lte'. apply bottom_perm_is_bottom.
-  - constructor; simpl; auto.
-Qed.
-
-(** * Recursive and reachability rules *)
-
-Lemma MuFold A G X `{FixedPoint G X} (F:PermType Si Ss A X -> PermType Si Ss A (G X))
-      {prp:Proper (lte_PermType _ _ ==> lte_PermType _ _) F}
-      xi xs :
-  xi :: F (mu _ _ F) ▷ xs ⊨ xi :: mu _ _ F ▷ foldFP xs.
-Proof.
-  (* FIXME: why can't we just rewrite with mu_fixed_point here? *)
-  eapply Proper_eq_Perms_lte_Perms; [ | reflexivity | ].
-  - apply Proper_eq_PermType_ptApp; [ apply mu_fixed_point | | ]; reflexivity.
-  - simpl. rewrite foldUnfold. reflexivity.
-Qed.
-
-Lemma MuUnfold A G X `{FixedPoint G X} (F:PermType Si Ss A X -> PermType Si Ss A (G X))
-      {prp:Proper (lte_PermType _ _ ==> lte_PermType _ _) F}
-      xi xs :
-   xi :: mu _ _ F ▷ xs ⊨ xi :: F (mu _ _ F) ▷ unfoldFP xs.
-Proof.
-  eapply Proper_eq_Perms_lte_Perms; [ reflexivity | | ].
-  - apply Proper_eq_PermType_ptApp; [ apply mu_fixed_point | | ]; reflexivity.
-  - simpl. reflexivity.
-Qed.
-
-(* Program Definition list_reach_perm r rw A (T : VPermType Si Ss A) : VPermType Si Ss (list A) := *)
-(*   @mu _ _ _ (mu_list A) _ (fixed_point_list _) *)
-(*       (fun U => or _ _ (eqp Si Ss r) ((ptr _ _ (rw, 0, T)) ⋆ (ptr _ _ (rw, 1, U)))) _. *)
-(* Next Obligation. *)
-(*   repeat intro. simpl. induction b; simpl in *; auto. *)
-(*   destruct H0 as (? & ? & ? & ? & ?). exists x0, x1. split; [| split]; auto. *)
-(*   clear H0. unfold ptr_Perms in *. destruct (offset a 1); auto. *)
-(*   destruct H1. destruct H0. destruct H0. subst. destruct H1 as (? & ? & ? & ? & ?). *)
-(*   eexists. split; eauto. do 2 eexists. split; eauto. split; eauto. apply H. auto. *)
-(* Qed. *)
-
-Lemma ReflR {A} x rw o (T : VPermType Si Ss A) :
-  x :: trueP _ _ ▷ tt ⊨ x :: reach_perm _ _ x rw o T ▷ nil.
-Proof.
-  repeat intro. apply mu_fixed_point. reflexivity.
-Qed.
-
-Lemma TransR {A} x y z rw o (T : VPermType Si Ss A) xs ys :
-  x :: reach_perm _ _ y rw o T ▷ xs * y :: reach_perm _ _ z rw o T ▷ ys ⊨
-  x :: reach_perm _ _ z rw o T ▷ (xs ++ ys).
-Proof.
-  revert x.
-  induction xs.
-  - intros x p (p1 & p2 & Hp1 & Hp2 & Hsep & Hlte).
-    destruct Hp1 as (? & (U & HU & ?) & Hp1); subst.
-    apply HU in Hp1. simpl in Hp1. subst. eapply Perms_upwards_closed; eauto.
-    etransitivity; eauto. apply lte_r_sep_conj_perm.
-  - intros x p (px' & py & Hpx' & Hpy & Hsep & Hlte).
-    eapply mu_fixed_point in Hpx'.
-    destruct Hpx' as (pa & px & Hpa & Hpx & Hsep' & Hlte').
-    (* x must be a pointer *)
-    destruct x; try contradiction. destruct a0 as [b o'].
-    destruct Hpx as (? & (v & ?) & Hpx); subst.
-    destruct Hpx as (px'' & pv & Hpx'' & Hpv & Hsep'' & Hlte'').
-
-    apply mu_fixed_point.
-    simpl.
-    exists pa. exists (px'' ** (pv ** py)). split; [apply Hpa | split; [| split]].
-    2: {
-        apply separate_sep_conj_perm.
-        - eapply separate_antimonotone; eauto.
-          etransitivity; eauto. apply lte_l_sep_conj_perm.
-        - apply separate_sep_conj_perm.
-          + eapply separate_antimonotone; eauto.
-            etransitivity; eauto. apply lte_r_sep_conj_perm.
-          + symmetry. symmetry in Hsep. eapply separate_antimonotone; eauto.
-            etransitivity; eauto. apply lte_l_sep_conj_perm.
-          + symmetry in Hsep. eapply separate_antimonotone; eauto.
-            etransitivity; eauto. etransitivity. apply lte_r_sep_conj_perm.
-            apply sep_conj_perm_monotone. reflexivity.
-            etransitivity; eauto. apply lte_r_sep_conj_perm.
-        - symmetry. apply separate_sep_conj_perm.
-          + eapply separate_antimonotone; eauto. reflexivity.
-          + symmetry. symmetry in Hsep. eapply separate_antimonotone; eauto.
-            etransitivity; eauto. etransitivity. apply lte_r_sep_conj_perm.
-            apply sep_conj_perm_monotone. reflexivity.
-            etransitivity; eauto. apply lte_l_sep_conj_perm.
-          + symmetry in Hsep. eapply separate_antimonotone; eauto.
-            etransitivity; eauto. etransitivity. apply lte_r_sep_conj_perm.
-            apply sep_conj_perm_monotone. reflexivity.
-            etransitivity; eauto. apply lte_r_sep_conj_perm.
-    }
-    2: { repeat rewrite <- sep_conj_perm_assoc.
-         etransitivity; eauto.
-         eapply sep_conj_perm_monotone; intuition.
-         repeat rewrite sep_conj_perm_assoc.
-         etransitivity; eauto.
-         eapply sep_conj_perm_monotone; intuition.
-    }
-    eexists. split; [eexists; reflexivity |].
-    apply sep_conj_Perms_perm; [apply Hpx'' | |].
-    2: {
-      apply separate_sep_conj_perm; auto.
-      + symmetry. symmetry in Hsep. eapply separate_antimonotone; eauto.
-        etransitivity; eauto. etransitivity. apply lte_r_sep_conj_perm.
-        apply sep_conj_perm_monotone. reflexivity.
-        etransitivity; eauto. apply lte_l_sep_conj_perm.
-      + symmetry in Hsep. eapply separate_antimonotone; eauto.
-        etransitivity; eauto. etransitivity. apply lte_r_sep_conj_perm.
-        apply sep_conj_perm_monotone. reflexivity.
-        etransitivity; eauto. apply lte_r_sep_conj_perm.
-    }
-    cbn. exists (v :: reach_perm _ _ z rw o T ▷ (xs ++ ys)). split.
-    2: {
-      apply IHxs. apply sep_conj_Perms_perm; auto.
-      symmetry. symmetry in Hsep. eapply separate_antimonotone; eauto.
-      etransitivity; eauto. etransitivity. apply lte_r_sep_conj_perm.
-      apply sep_conj_perm_monotone. reflexivity.
-      etransitivity; eauto. apply lte_r_sep_conj_perm.
-    }
-    eexists; split; eauto.
-    repeat intro. eapply mu_fixed_point in H0; auto.
-    Unshelve. all: apply reach_perm_proper.
-Qed.
-
-(*
+  (*
    while (v != NULL)
          v = *(v + 1);
    return 0;
-*)
+   *)
+  (*
 Definition ex3i' : Value -> itree (sceE Si) Value :=
   iter (C := Kleisli _)
        (fun v =>  b <- isNull v;;
@@ -1275,7 +402,7 @@ Qed.
         v = *(v + 1);
         n++;
   }
-*)
+   *)
 Definition ex3i (v : Value) : itree (sceE Si) Value :=
   iter (C := Kleisli _)
        (fun '(n, v) => b <- isNull v;;
@@ -1324,3 +451,5 @@ Proof.
   - intros []. admit.
   - intros [a ys]. admit.
 Abort.
+   *)
+End Rules.
