src/Temporal.v
@@ -1,6 +1,7 @@
 (* begin hide *)
 
 From Heapster Require Import
+     Utils
      Permissions
      SepStep
      Typing.
